@prefix : <https://w3id.org/whow/onto/hydrography/> .
@prefix dc: <http://purl.org/dc/elements/1.1/> .
@prefix dct: <http://purl.org/dc/terms/> .
@prefix owl: <http://www.w3.org/2002/07/owl#> .
@prefix rdf: <http://www.w3.org/1999/02/22-rdf-syntax-ns#> .
@prefix xml: <http://www.w3.org/XML/1998/namespace> .
@prefix xsd: <http://www.w3.org/2001/XMLSchema#> .
@prefix prov: <http://www.w3.org/ns/prov#> .
@prefix rdfs: <http://www.w3.org/2000/01/rdf-schema#> .
@prefix ispra-emf: <https://w3id.org/italia/env/onto/inspire-mf/> .
@base <https://w3id.org/whow/onto/hydrography> .

<https://w3id.org/whow/onto/hydrography> rdf:type owl:Ontology ;
                                          owl:versionIRI <https://w3id.org/whow/onto/hydrography/0.2> ;
                                          dc:description <https://raw.githubusercontent.com/whow-project/semantic-assets/main/ontologies/graphical-representation-ontologies/hydrography-ontology.png> ;
                                          dct:description "Ontologia per la descrizione dell'idrografia. Include concetti quali i bacini idrici e la classificazione dei corpi idrici. È semanticamente allineata a concetti definiti nell'INSPIRE registry."@it ,
                                                          "Ontology for describing the hydrography. It includes concepts such as water basins and the classification of water bodies"@en ;
                                          dct:modified "2023-02-13"^^xsd:date ;
                                          dct:issued "2022-01-10"^^xsd:date ;
                                          dct:title "Hydrography Ontology"@en ,
                                                    "Ontologia dell'Idrografia"@it ;
                                          rdfs:comment "Ontologia per la descrizione dell'idrografia. Include concetti quali i bacini idrici e la classificazione dei corpi idrici. È semanticamente allineata a concetti definiti nell'INSPIRE registry."@it ,
                                                       "Ontology for describing the hydrography. It includes concepts such as water basins and the classification of water bodies"@en ;
                                          rdfs:label "Hydrography Ontology"@en ;
                                          owl:versionInfo "version 0.2 - refactor URI of imported concept"@en .

#################################################################
#    Annotation properties
#################################################################

###  http://purl.org/dc/elements/1.1/description
dc:description rdf:type owl:AnnotationProperty .


###  http://purl.org/dc/terms/description
dct:description rdf:type owl:AnnotationProperty .


###  http://purl.org/dc/terms/modified
dct:modified rdf:type owl:AnnotationProperty .


###  http://purl.org/dc/terms/title
dct:title rdf:type owl:AnnotationProperty .


###  http://www.w3.org/ns/prov#wasDerivedFrom
prov:wasDerivedFrom rdf:type owl:AnnotationProperty .


#################################################################
#    Object Properties
#################################################################

###  https://w3id.org/whow/onto/hydrography/belongsToWaterBasin
:belongsToWaterBasin rdf:type owl:ObjectProperty ;
                     rdfs:domain :WaterBody ;
                     rdfs:range :WaterBasin ;
                     rdfs:comment "This property links the water body to the water basin it belongs"@en ;
                     rdfs:label "belongs to water basin"@en .


###  https://w3id.org/whow/onto/hydrography/isSubWaterBasin
:isSubWaterBasin rdf:type owl:ObjectProperty ;
                 rdfs:domain :WaterBasin ;
                 rdfs:range :WaterBasin ;
                 rdfs:comment "This property is used to represent hierarchies of water basin since water basins can be formed by other water basins."@en ;
                 rdfs:label "is sub water basin"@en .


#################################################################
#    Classes
#################################################################

###  https://w3id.org/italia/env/onto/inspire-emf/FeatureOfInterest
<https://w3id.org/italia/env/onto/inspire-emf/FeatureOfInterest> rdf:type owl:Class .


###  https://w3id.org/whow/onto/hydrography/CoastalWaterBody
:CoastalWaterBody rdf:type owl:Class ;
                  rdfs:subClassOf :WaterBody ;
                  rdfs:comment "The class of coastal water body; that is, a marine water body bordering a coast"@en ;
                  rdfs:isDefinedBy <https://w3id.org/whow/onto/hydrography> ;
                  rdfs:label "Coastal Water Body"@en ;
                  prov:wasDerivedFrom <http://inspire.ec.europa.eu/featureconcept/WFDCoastalWater> .


###  https://w3id.org/whow/onto/hydrography/GroundwaterBody
:GroundwaterBody rdf:type owl:Class ;
                 rdfs:subClassOf :WaterBody ;
                 rdfs:comment "A distinct volume of groundwater within an aquifer or system of aquifers, which is hydraulically isolated from nearby groundwater bodies."@en ;
                 rdfs:isDefinedBy <https://w3id.org/whow/onto/hydrography> ;
                 rdfs:label "Groundwater Body"@en ;
                 prov:wasDerivedFrom <http://inspire.ec.europa.eu/featureconcept/GroundWaterBody> .


###  https://w3id.org/whow/onto/hydrography/LakeWaterBody
:LakeWaterBody rdf:type owl:Class ;
               rdfs:subClassOf :WaterBody ;
               rdfs:comment "A body of standing inland surface water."@en ;
               rdfs:isDefinedBy <https://w3id.org/whow/onto/hydrography> ;
               rdfs:label "Lake Water Body"@en ;
               prov:wasDerivedFrom <http://inspire.ec.europa.eu/featureconcept/WFDLake> .


###  https://w3id.org/whow/onto/hydrography/MarineWater
:MarineWater rdf:type owl:Class ;
             rdfs:subClassOf :WaterBody ;
             rdfs:comment "The waters, the seabed and subsoil on the seaward side of the baseline from which the extent of territorial waters is measured"@en ;
             rdfs:isDefinedBy <https://w3id.org/whow/onto/hydrography> ;
             rdfs:label "Marine Water"@en .


###  https://w3id.org/whow/onto/hydrography/RiverWaterBody
:RiverWaterBody rdf:type owl:Class ;
                rdfs:subClassOf :WaterBody ;
                rdfs:comment "A body of inland water flowing for the most part on the surface of the land but which may flow underground for part of its course."@en ;
                rdfs:isDefinedBy <https://w3id.org/whow/onto/hydrography> ;
                rdfs:label "River Water Body"@en ;
                prov:wasDerivedFrom <http://inspire.ec.europa.eu/featureconcept/WFDRiver> .


###  https://w3id.org/whow/onto/hydrography/TransitionalWaterBody
:TransitionalWaterBody rdf:type owl:Class ;
                       rdfs:subClassOf :WaterBody ;
                       rdfs:comment "Bodies of surface water in the vicinity of river mouths which are partly saline in character as a result of their proximity to coastal waters but which are substantially influenced by freshwater flows."@en ;
                       rdfs:isDefinedBy <https://w3id.org/whow/onto/hydrography> ;
                       rdfs:label "Transitional Water Body"@en ;
                       prov:wasDerivedFrom <http://inspire.ec.europa.eu/featureconcept/WFDTransitionalWater> .


###  https://w3id.org/whow/onto/hydrography/WaterBasin
:WaterBasin rdf:type owl:Class ;
            rdfs:subClassOf :WaterFeature ,
                            [ rdf:type owl:Restriction ;
                              owl:onProperty :isSubWaterBasin ;
                              owl:allValuesFrom :WaterBasin
                            ] ;
            rdfs:isDefinedBy <https://w3id.org/whow/onto/hydrography> ;
            rdfs:label "Water Basin"@en .


###  https://w3id.org/whow/onto/hydrography/WaterBody
:WaterBody rdf:type owl:Class ;
           rdfs:subClassOf :WaterFeature ,
                           [ rdf:type owl:Restriction ;
                             owl:onProperty :belongsToWaterBasin ;
                             owl:someValuesFrom :WaterBasin
                           ] ,
                           [ rdf:type owl:Restriction ;
                             owl:onProperty :belongsToWaterBasin ;
                             owl:allValuesFrom :WaterBasin
                           ] ;
           rdfs:comment "Abstract class representing a WFD - Water Framework Directive body of surface water or body of groundwater"@en ;
           rdfs:isDefinedBy <https://w3id.org/whow/onto/hydrography> ;
           rdfs:label "Water Body"@en ;
           prov:wasDerivedFrom <http://inspire.ec.europa.eu/featureconcept/WFDWaterBody> .


###  https://w3id.org/whow/onto/hydrography/WaterFeature
:WaterFeature rdf:type owl:Class ;
              rdfs:subClassOf <https://w3id.org/italia/env/onto/inspire-emf/FeatureOfInterest> ;
              rdfs:comment "A specific feature of interest in the hydrography context."@en ;
              rdfs:isDefinedBy <https://w3id.org/whow/onto/hydrography> ;
              rdfs:label "Water Feature"@en .


###  Generated by the OWL API (version 4.5.9.2019-02-01T07:24:44Z) https://github.com/owlcs/owlapi
