<?xml version="1.0"?>
<rdf:RDF xmlns="https://w3id.org/whow/onto/hydrography/"
     xml:base="https://w3id.org/whow/onto/hydrography/"
     xmlns:dc="http://purl.org/dc/elements/1.1/"
     xmlns:dct="http://purl.org/dc/terms/"
     xmlns:owl="http://www.w3.org/2002/07/owl#"
     xmlns:rdf="http://www.w3.org/1999/02/22-rdf-syntax-ns#"
     xmlns:xml="http://www.w3.org/XML/1998/namespace"
     xmlns:xsd="http://www.w3.org/2001/XMLSchema#"
     xmlns:prov="http://www.w3.org/ns/prov#"
     xmlns:rdfs="http://www.w3.org/2000/01/rdf-schema#"
     xmlns:ispra-emf="https://w3id.org/italia/env/onto/inspire-mf/">
    <owl:Ontology rdf:about="https://w3id.org/whow/onto/hydrography">
        <owl:versionIRI rdf:resource="https://w3id.org/whow/onto/hydrography/0.2"/>
        <dc:description rdf:resource="https://raw.githubusercontent.com/whow-project/semantic-assets/main/ontologies/graphical-representation-ontologies/hydrography-ontology.png"/>
        <dct:description xml:lang="it">Ontologia per la descrizione dell&apos;idrografia. Include concetti quali i bacini idrici e la classificazione dei corpi idrici. È semanticamente allineata a concetti definiti nell&apos;INSPIRE registry.</dct:description>
        <dct:description xml:lang="en">Ontology for describing the hydrography. It includes concepts such as water basins and the classification of water bodies</dct:description>
        <dct:modified rdf:datatype="http://www.w3.org/2001/XMLSchema#date">2023-11-08</dct:modified>
        <dct:issued rdf:datatype="http://www.w3.org/2001/XMLSchema#date">2022-01-10</dct:issued>
        <dct:title xml:lang="en">Hydrography Ontology</dct:title>
        <dct:title xml:lang="it">Ontologia dell&apos;Idrografia</dct:title>
        <rdfs:comment xml:lang="it">Ontologia per la descrizione dell&apos;idrografia. Include concetti quali i bacini idrici e la classificazione dei corpi idrici. È semanticamente allineata a concetti definiti nell&apos;INSPIRE registry.</rdfs:comment>
        <rdfs:comment xml:lang="en">Ontology for describing the hydrography. It includes concepts such as water basins and the classification of water bodies</rdfs:comment>
        <rdfs:label xml:lang="en">Hydrography Ontology</rdfs:label>
        <owl:versionInfo xml:lang="en">version 0.2 - refactor URI of imported concept</owl:versionInfo>
    </owl:Ontology>



    <!--
    ///////////////////////////////////////////////////////////////////////////////////////
    //
    // Annotation properties
    //
    ///////////////////////////////////////////////////////////////////////////////////////
     -->




    <!-- http://purl.org/dc/elements/1.1/description -->

    <owl:AnnotationProperty rdf:about="http://purl.org/dc/elements/1.1/description"/>



    <!-- http://purl.org/dc/terms/description -->

    <owl:AnnotationProperty rdf:about="http://purl.org/dc/terms/description"/>



    <!-- http://purl.org/dc/terms/modified -->

    <owl:AnnotationProperty rdf:about="http://purl.org/dc/terms/modified"/>



    <!-- http://purl.org/dc/terms/title -->

    <owl:AnnotationProperty rdf:about="http://purl.org/dc/terms/title"/>



    <!-- http://www.w3.org/ns/prov#wasDerivedFrom -->

    <owl:AnnotationProperty rdf:about="http://www.w3.org/ns/prov#wasDerivedFrom"/>



    <!--
    ///////////////////////////////////////////////////////////////////////////////////////
    //
    // Object Properties
    //
    ///////////////////////////////////////////////////////////////////////////////////////
     -->




    <!-- https://w3id.org/whow/onto/hydrography/belongsToWaterBasin -->

    <owl:ObjectProperty rdf:about="https://w3id.org/whow/onto/hydrography/belongsToWaterBasin">
        <rdfs:domain rdf:resource="https://w3id.org/whow/onto/hydrography/WaterBody"/>
        <rdfs:range rdf:resource="https://w3id.org/whow/onto/hydrography/WaterBasin"/>
        <rdfs:comment xml:lang="en">This property links the water body to the water basin it belongs</rdfs:comment>
        <rdfs:label xml:lang="en">belongs to water basin</rdfs:label>
    </owl:ObjectProperty>



    <!-- https://w3id.org/whow/onto/hydrography/isSubWaterBasin -->

    <owl:ObjectProperty rdf:about="https://w3id.org/whow/onto/hydrography/isSubWaterBasin">
        <rdfs:domain rdf:resource="https://w3id.org/whow/onto/hydrography/WaterBasin"/>
        <rdfs:range rdf:resource="https://w3id.org/whow/onto/hydrography/WaterBasin"/>
        <rdfs:comment xml:lang="en">This property is used to represent hierarchies of water basin since water basins can be formed by other water basins.</rdfs:comment>
        <rdfs:label xml:lang="en">is sub water basin</rdfs:label>
    </owl:ObjectProperty>



    <!--
    ///////////////////////////////////////////////////////////////////////////////////////
    //
    // Classes
    //
    ///////////////////////////////////////////////////////////////////////////////////////
     -->




    <!-- https://w3id.org/italia/env/onto/inspire-emf/FeatureOfInterest -->

    <owl:Class rdf:about="https://w3id.org/italia/env/onto/inspire-emf/FeatureOfInterest"/>



    <!-- https://w3id.org/whow/onto/hydrography/CoastalWaterBody -->

    <owl:Class rdf:about="https://w3id.org/whow/onto/hydrography/CoastalWaterBody">
        <rdfs:subClassOf rdf:resource="https://w3id.org/whow/onto/hydrography/WaterBody"/>
        <rdfs:comment xml:lang="en">The class of coastal water body; that is, a marine water body bordering a coast</rdfs:comment>
        <rdfs:isDefinedBy rdf:resource="https://w3id.org/whow/onto/hydrography"/>
        <rdfs:label xml:lang="en">Coastal Water Body</rdfs:label>
        <prov:wasDerivedFrom rdf:resource="http://inspire.ec.europa.eu/featureconcept/WFDCoastalWater"/>
    </owl:Class>



    <!-- https://w3id.org/whow/onto/hydrography/GroundwaterBody -->

    <owl:Class rdf:about="https://w3id.org/whow/onto/hydrography/GroundwaterBody">
        <rdfs:subClassOf rdf:resource="https://w3id.org/whow/onto/hydrography/WaterBody"/>
        <rdfs:comment xml:lang="en">A distinct volume of groundwater within an aquifer or system of aquifers, which is hydraulically isolated from nearby groundwater bodies.</rdfs:comment>
        <rdfs:isDefinedBy rdf:resource="https://w3id.org/whow/onto/hydrography"/>
        <rdfs:label xml:lang="en">Groundwater Body</rdfs:label>
        <prov:wasDerivedFrom rdf:resource="http://inspire.ec.europa.eu/featureconcept/GroundWaterBody"/>
    </owl:Class>



    <!-- https://w3id.org/whow/onto/hydrography/LakeWaterBody -->

    <owl:Class rdf:about="https://w3id.org/whow/onto/hydrography/LakeWaterBody">
        <rdfs:subClassOf rdf:resource="https://w3id.org/whow/onto/hydrography/WaterBody"/>
        <rdfs:comment xml:lang="en">A body of standing inland surface water.</rdfs:comment>
        <rdfs:isDefinedBy rdf:resource="https://w3id.org/whow/onto/hydrography"/>
        <rdfs:label xml:lang="en">Lake Water Body</rdfs:label>
        <prov:wasDerivedFrom rdf:resource="http://inspire.ec.europa.eu/featureconcept/WFDLake"/>
    </owl:Class>



    <!-- https://w3id.org/whow/onto/hydrography/MarineWaterBody -->

    <owl:Class rdf:about="https://w3id.org/whow/onto/hydrography/MarineWaterBody">
        <rdfs:subClassOf rdf:resource="https://w3id.org/whow/onto/hydrography/WaterBody"/>
        <rdfs:comment xml:lang="en">The waters, the seabed and subsoil on the seaward side of the baseline from which the extent of territorial waters is measured</rdfs:comment>
        <rdfs:isDefinedBy rdf:resource="https://w3id.org/whow/onto/hydrography"/>
        <rdfs:label xml:lang="en">Marine Water</rdfs:label>
    </owl:Class>



    <!-- https://w3id.org/whow/onto/hydrography/RiverWaterBody -->

    <owl:Class rdf:about="https://w3id.org/whow/onto/hydrography/RiverWaterBody">
        <rdfs:subClassOf rdf:resource="https://w3id.org/whow/onto/hydrography/WaterBody"/>
        <rdfs:comment xml:lang="en">A body of inland water flowing for the most part on the surface of the land but which may flow underground for part of its course.</rdfs:comment>
        <rdfs:isDefinedBy rdf:resource="https://w3id.org/whow/onto/hydrography"/>
        <rdfs:label xml:lang="en">River Water Body</rdfs:label>
        <prov:wasDerivedFrom rdf:resource="http://inspire.ec.europa.eu/featureconcept/WFDRiver"/>
    </owl:Class>



    <!-- https://w3id.org/whow/onto/hydrography/TransitionalWaterBody -->

    <owl:Class rdf:about="https://w3id.org/whow/onto/hydrography/TransitionalWaterBody">
        <rdfs:subClassOf rdf:resource="https://w3id.org/whow/onto/hydrography/WaterBody"/>
        <rdfs:comment xml:lang="en">Bodies of surface water in the vicinity of river mouths which are partly saline in character as a result of their proximity to coastal waters but which are substantially influenced by freshwater flows.</rdfs:comment>
        <rdfs:isDefinedBy rdf:resource="https://w3id.org/whow/onto/hydrography"/>
        <rdfs:label xml:lang="en">Transitional Water Body</rdfs:label>
        <prov:wasDerivedFrom rdf:resource="http://inspire.ec.europa.eu/featureconcept/WFDTransitionalWater"/>
    </owl:Class>



    <!-- https://w3id.org/whow/onto/hydrography/WaterBasin -->

    <owl:Class rdf:about="https://w3id.org/whow/onto/hydrography/WaterBasin">
        <rdfs:subClassOf rdf:resource="https://w3id.org/whow/onto/hydrography/WaterFeature"/>
        <rdfs:subClassOf>
            <owl:Restriction>
                <owl:onProperty rdf:resource="https://w3id.org/whow/onto/hydrography/isSubWaterBasin"/>
                <owl:allValuesFrom rdf:resource="https://w3id.org/whow/onto/hydrography/WaterBasin"/>
            </owl:Restriction>
        </rdfs:subClassOf>
        <rdfs:isDefinedBy rdf:resource="https://w3id.org/whow/onto/hydrography"/>
        <rdfs:label xml:lang="en">Water Basin</rdfs:label>
    </owl:Class>



    <!-- https://w3id.org/whow/onto/hydrography/WaterBody -->

    <owl:Class rdf:about="https://w3id.org/whow/onto/hydrography/WaterBody">
        <rdfs:subClassOf rdf:resource="https://w3id.org/whow/onto/hydrography/WaterFeature"/>
        <rdfs:subClassOf>
            <owl:Restriction>
                <owl:onProperty rdf:resource="https://w3id.org/whow/onto/hydrography/belongsToWaterBasin"/>
                <owl:someValuesFrom rdf:resource="https://w3id.org/whow/onto/hydrography/WaterBasin"/>
            </owl:Restriction>
        </rdfs:subClassOf>
        <rdfs:subClassOf>
            <owl:Restriction>
                <owl:onProperty rdf:resource="https://w3id.org/whow/onto/hydrography/belongsToWaterBasin"/>
                <owl:allValuesFrom rdf:resource="https://w3id.org/whow/onto/hydrography/WaterBasin"/>
            </owl:Restriction>
        </rdfs:subClassOf>
        <rdfs:comment xml:lang="en">Abstract class representing a WFD - Water Framework Directive body of surface water or body of groundwater</rdfs:comment>
        <rdfs:isDefinedBy rdf:resource="https://w3id.org/whow/onto/hydrography"/>
        <rdfs:label xml:lang="en">Water Body</rdfs:label>
        <prov:wasDerivedFrom rdf:resource="http://inspire.ec.europa.eu/featureconcept/WFDWaterBody"/>
    </owl:Class>



    <!-- https://w3id.org/whow/onto/hydrography/WaterFeature -->

    <owl:Class rdf:about="https://w3id.org/whow/onto/hydrography/WaterFeature">
        <rdfs:subClassOf rdf:resource="https://w3id.org/italia/env/onto/inspire-emf/FeatureOfInterest"/>
        <rdfs:comment xml:lang="en">A specific feature of interest in the hydrography context.</rdfs:comment>
        <rdfs:isDefinedBy rdf:resource="https://w3id.org/whow/onto/hydrography"/>
        <rdfs:label xml:lang="en">Water Feature</rdfs:label>
    </owl:Class>
</rdf:RDF>



<!-- Generated by the OWL API (version 4.5.9.2019-02-01T07:24:44Z) https://github.com/owlcs/owlapi -->
