<?xml version="1.0"?>
<rdf:RDF xmlns="http://www.w3id.com/whow/onto/weather-monitoring"
     xml:base="http://www.w3id.com/whow/onto/weather-monitoring"
     xmlns:dc="http://purl.org/dc/elements/1.1/"
     xmlns:dct="http://purl.org/dc/terms/"
     xmlns:owl="http://www.w3.org/2002/07/owl#"
     xmlns:rdf="http://www.w3.org/1999/02/22-rdf-syntax-ns#"
     xmlns:xml="http://www.w3.org/XML/1998/namespace"
     xmlns:xsd="http://www.w3.org/2001/XMLSchema#"
     xmlns:rdfs="http://www.w3.org/2000/01/rdf-schema#">
    <owl:Ontology rdf:about="http://www.w3id.com/whow/onto/weather-monitoring">
        <owl:imports rdf:resource="https://w3id.org/italia/env/onto/inspire-mf/"/>
        <owl:imports rdf:resource="https://w3id.org/italia/env/onto/place/"/>
        <dc:description rdf:resource="https://raw.githubusercontent.com/whow-project/semantic-assets/main/ontologies/images/weather-monitoring.png"/>
        <dct:issued rdf:datatype="http://www.w3.org/2001/XMLSchema#date">2023-01-30</dct:issued>
        <dct:modified rdf:datatype="http://www.w3.org/2001/XMLSchema#date">2023-01-30</dct:modified>
        <rdfs:label xml:lang="it">Ontologia per il monitoraggio meteo</rdfs:label>
        <rdfs:label xml:lang="en">Weather Monitoring Ontology</rdfs:label>
    </owl:Ontology>
    


    <!-- 
    ///////////////////////////////////////////////////////////////////////////////////////
    //
    // Annotation properties
    //
    ///////////////////////////////////////////////////////////////////////////////////////
     -->

    


    <!-- http://purl.org/dc/elements/1.1/description -->

    <owl:AnnotationProperty rdf:about="http://purl.org/dc/elements/1.1/description"/>
    


    <!-- http://purl.org/dc/terms/issued -->

    <owl:AnnotationProperty rdf:about="http://purl.org/dc/terms/issued"/>
    


    <!-- http://purl.org/dc/terms/modified -->

    <owl:AnnotationProperty rdf:about="http://purl.org/dc/terms/modified"/>
    


    <!-- 
    ///////////////////////////////////////////////////////////////////////////////////////
    //
    // Object Properties
    //
    ///////////////////////////////////////////////////////////////////////////////////////
     -->

    


    <!-- http://www.w3id.com/whow/onto/weather-monitoring/hasObservedWeatherProperty -->

    <owl:ObjectProperty rdf:about="http://www.w3id.com/whow/onto/weather-monitoring/hasObservedWeatherProperty">
        <rdfs:subPropertyOf rdf:resource="https://w3id.org/italia/env/onto/inspire-mf/hasObservationParameter"/>
        <rdfs:domain rdf:resource="http://www.w3id.com/whow/onto/weather-monitoring/WeatherObservation"/>
        <rdfs:range rdf:resource="http://www.w3id.com/whow/onto/weather-monitoring/WeatherObservableProperty"/>
        <rdfs:comment xml:lang="en">Property that links the weather observation to its weather property (e.g., global radiation, temperature, etc.)</rdfs:comment>
        <rdfs:comment xml:lang="it">Proprietà che collega l&apos;osservazione meteorologica alla sua proprietà meteorologica osservata (e.g., radiazione globale, temperatura, precipazione, ecc.)</rdfs:comment>
        <rdfs:isDefinedBy rdf:resource="http://www.w3id.com/whow/onto/weather-monitoring"/>
        <rdfs:label xml:lang="it">ha proprietà meteorologica osservata</rdfs:label>
        <rdfs:label xml:lang="en">has observed weather property</rdfs:label>
        <owl:versionInfo xml:lang="it">stabile</owl:versionInfo>
        <owl:versionInfo xml:lang="en">stable</owl:versionInfo>
    </owl:ObjectProperty>
    


    <!-- http://www.w3id.com/whow/onto/weather-monitoring/hasResultTime -->

    <owl:ObjectProperty rdf:about="http://www.w3id.com/whow/onto/weather-monitoring/hasResultTime">
        <rdfs:subPropertyOf rdf:resource="https://w3id.org/italia/env/onto/top/atTime"/>
        <rdfs:domain rdf:resource="http://www.w3id.com/whow/onto/weather-monitoring/WeatherObservation"/>
        <rdfs:range rdf:resource="https://w3id.orgitalia/onto/TI/TimeInstant"/>
        <rdfs:comment xml:lang="en">Property used to model the time instant in which the (weather) observation is done.</rdfs:comment>
        <rdfs:comment xml:lang="it">Proprietà utilizzata per modellare l&apos;istante temporale in cui viene fatta l&apos;osservazione (meteorologica).</rdfs:comment>
        <rdfs:isDefinedBy rdf:resource="http://www.w3id.com/whow/onto/weather-monitoring"/>
        <rdfs:label xml:lang="it">ha tempo del risultato</rdfs:label>
        <rdfs:label xml:lang="en">has result time</rdfs:label>
        <owl:versionInfo xml:lang="it">provvisorio</owl:versionInfo>
        <owl:versionInfo xml:lang="en">unstable</owl:versionInfo>
    </owl:ObjectProperty>
    


    <!-- http://www.w3id.com/whow/onto/weather-monitoring/hasValidityPeriod -->

    <owl:ObjectProperty rdf:about="http://www.w3id.com/whow/onto/weather-monitoring/hasValidityPeriod">
        <rdfs:domain rdf:resource="http://www.w3id.com/whow/onto/weather-monitoring/WeatherSensor"/>
        <rdfs:range rdf:resource="https://w3id.org/italia/env/onto/top/TimeInterval"/>
        <rdfs:comment xml:lang="en">Property used to model a period of time of validity of a sensor</rdfs:comment>
        <rdfs:comment xml:lang="en">Proprietà utilizzata per modellare un periodo di tempo di validità di un sensore</rdfs:comment>
        <rdfs:isDefinedBy rdf:resource="http://www.w3id.com/whow/onto/weather-monitoring"/>
        <rdfs:label xml:lang="it">ha periodo di validità</rdfs:label>
        <rdfs:label xml:lang="en">has validity period</rdfs:label>
        <owl:versionInfo xml:lang="it">stabile</owl:versionInfo>
        <owl:versionInfo xml:lang="en">stable</owl:versionInfo>
    </owl:ObjectProperty>
    


    <!-- http://www.w3id.com/whow/onto/weather-monitoring/hasWeatherFeatureOfInterest -->

    <owl:ObjectProperty rdf:about="http://www.w3id.com/whow/onto/weather-monitoring/hasWeatherFeatureOfInterest">
        <rdfs:subPropertyOf rdf:resource="https://w3id.org/italia/env/onto/inspire-mf/hasFeatureOfInterest"/>
        <rdfs:domain rdf:resource="http://www.w3id.com/whow/onto/weather-monitoring/WeatherObservation"/>
        <rdfs:range rdf:resource="http://www.w3id.com/whow/onto/weather-monitoring/WeatherFeatureOfInterest"/>
        <rdfs:comment xml:lang="en">Property that links a meteorological observation to its meteorological characteristic of interest. Example: If the observed property is &apos;precipitation&apos; then the meteorological observation can be linked to rainfall as a characteristic of interest.</rdfs:comment>
        <rdfs:comment xml:lang="it">Proprietà che collega un&apos;osservazione meteorologica alla propria caratteristica di interesse meteorologica. Esempio: se la proprietà osservata è la precipitazione allora l&apos;osservazione meteorologica può essere collegata alla pioggia come caratteristica di interesse.</rdfs:comment>
        <rdfs:isDefinedBy rdf:resource="http://www.w3id.com/whow/onto/weather-monitoring"/>
        <rdfs:label xml:lang="it">ha caratteristica di interesse meteorologica</rdfs:label>
        <rdfs:label xml:lang="en">has weather feature of interest</rdfs:label>
        <owl:versionInfo xml:lang="it">stabile</owl:versionInfo>
        <owl:versionInfo xml:lang="en">stable</owl:versionInfo>
    </owl:ObjectProperty>
    


    <!-- https://w3id.org/italia/env/onto/inspire-mf/hasFeatureOfInterest -->

    <owl:ObjectProperty rdf:about="https://w3id.org/italia/env/onto/inspire-mf/hasFeatureOfInterest"/>
    


    <!-- https://w3id.org/italia/env/onto/inspire-mf/hasObservationParameter -->

    <owl:ObjectProperty rdf:about="https://w3id.org/italia/env/onto/inspire-mf/hasObservationParameter"/>
    


    <!-- https://w3id.org/italia/env/onto/inspire-mf/hasSensorType -->

    <owl:ObjectProperty rdf:about="https://w3id.org/italia/env/onto/inspire-mf/hasSensorType"/>
    


    <!-- https://w3id.org/italia/env/onto/inspire-mf/isHostedBy -->

    <owl:ObjectProperty rdf:about="https://w3id.org/italia/env/onto/inspire-mf/isHostedBy"/>
    


    <!-- https://w3id.org/italia/env/onto/inspire-mf/isObservationMadeBySensor -->

    <owl:ObjectProperty rdf:about="https://w3id.org/italia/env/onto/inspire-mf/isObservationMadeBySensor"/>
    


    <!-- https://w3id.org/italia/env/onto/place/hasGeometry -->

    <owl:ObjectProperty rdf:about="https://w3id.org/italia/env/onto/place/hasGeometry"/>
    


    <!-- https://w3id.org/italia/env/onto/top/atTime -->

    <owl:ObjectProperty rdf:about="https://w3id.org/italia/env/onto/top/atTime"/>
    


    <!-- 
    ///////////////////////////////////////////////////////////////////////////////////////
    //
    // Classes
    //
    ///////////////////////////////////////////////////////////////////////////////////////
     -->

    


    <!-- http://www.w3id.com/whow/onto/weather-monitoring/WeatherFeatureOfInterest -->

    <owl:Class rdf:about="http://www.w3id.com/whow/onto/weather-monitoring/WeatherFeatureOfInterest">
        <rdfs:subClassOf rdf:resource="https://w3id.org/italia/env/onto/inspire-mf/FeatureOfInterest"/>
        <rdfs:comment xml:lang="it">La classe delle caratteristiche di interesse per il meteo. Esempi includono: aria, pioggia, livello del suolo, neve, ecc.</rdfs:comment>
        <rdfs:comment xml:lang="en">The class of feature of interest specific for the meteo domain. Examples include: Air, Wind, Rainfall, Snow, etc.</rdfs:comment>
        <rdfs:isDefinedBy rdf:resource="http://www.w3id.com/whow/onto/weather-monitoring"/>
        <rdfs:label xml:lang="it">Caratteristica di Interesse Meteorologica</rdfs:label>
        <rdfs:label xml:lang="en">Weather Feature of Interest</rdfs:label>
        <owl:versionInfo xml:lang="it">stabile</owl:versionInfo>
        <owl:versionInfo xml:lang="en">stable</owl:versionInfo>
    </owl:Class>
    


    <!-- http://www.w3id.com/whow/onto/weather-monitoring/WeatherObservableProperty -->

    <owl:Class rdf:about="http://www.w3id.com/whow/onto/weather-monitoring/WeatherObservableProperty">
        <rdfs:subClassOf rdf:resource="https://w3id.org/italia/env/onto/inspire-mf/ObservationParameter"/>
        <rdfs:comment xml:lang="it">La classe di tutte le possibile proprietà osservabili relative alle rilevazioni meteorologiche. Per esempio, sono proprietà osservabili le precipitazioni, la radiazione globale, la temperatura dell&apos;aria, l&apos;altezza della neve, ecc.</rdfs:comment>
        <rdfs:comment xml:lang="en">The class of all the possible weather observable properties. Examples include: global radiation, the quantity of rainfall, the temperature of the air,, the level of snow, etc.</rdfs:comment>
        <rdfs:isDefinedBy rdf:resource="http://www.w3id.com/whow/onto/weather-monitoring"/>
        <rdfs:label xml:lang="it">Proprietà Meteorologica Osservabile</rdfs:label>
        <rdfs:label xml:lang="en">Weather Observable Property</rdfs:label>
        <owl:versionInfo xml:lang="it">stabile</owl:versionInfo>
        <owl:versionInfo xml:lang="en">stable</owl:versionInfo>
    </owl:Class>
    


    <!-- http://www.w3id.com/whow/onto/weather-monitoring/WeatherObservation -->

    <owl:Class rdf:about="http://www.w3id.com/whow/onto/weather-monitoring/WeatherObservation">
        <rdfs:subClassOf rdf:resource="https://w3id.org/italia/env/onto/inspire-mf/Observation"/>
        <rdfs:subClassOf>
            <owl:Restriction>
                <owl:onProperty rdf:resource="http://www.w3id.com/whow/onto/weather-monitoring/hasObservedWeatherProperty"/>
                <owl:allValuesFrom rdf:resource="http://www.w3id.com/whow/onto/weather-monitoring/WeatherObservableProperty"/>
            </owl:Restriction>
        </rdfs:subClassOf>
        <rdfs:subClassOf>
            <owl:Restriction>
                <owl:onProperty rdf:resource="http://www.w3id.com/whow/onto/weather-monitoring/hasWeatherFeatureOfInterest"/>
                <owl:allValuesFrom rdf:resource="http://www.w3id.com/whow/onto/weather-monitoring/WeatherFeatureOfInterest"/>
            </owl:Restriction>
        </rdfs:subClassOf>
        <rdfs:subClassOf>
            <owl:Restriction>
                <owl:onProperty rdf:resource="http://www.w3id.com/whow/onto/weather-monitoring/hasObservedWeatherProperty"/>
                <owl:qualifiedCardinality rdf:datatype="http://www.w3.org/2001/XMLSchema#nonNegativeInteger">1</owl:qualifiedCardinality>
                <owl:onClass rdf:resource="http://www.w3id.com/whow/onto/weather-monitoring/WeatherObservableProperty"/>
            </owl:Restriction>
        </rdfs:subClassOf>
        <rdfs:subClassOf>
            <owl:Restriction>
                <owl:onProperty rdf:resource="http://www.w3id.com/whow/onto/weather-monitoring/hasResultTime"/>
                <owl:qualifiedCardinality rdf:datatype="http://www.w3.org/2001/XMLSchema#nonNegativeInteger">1</owl:qualifiedCardinality>
                <owl:onClass rdf:resource="https://w3id.orgitalia/onto/TI/TimeInstant"/>
            </owl:Restriction>
        </rdfs:subClassOf>
        <rdfs:subClassOf>
            <owl:Restriction>
                <owl:onProperty rdf:resource="http://www.w3id.com/whow/onto/weather-monitoring/hasWeatherFeatureOfInterest"/>
                <owl:qualifiedCardinality rdf:datatype="http://www.w3.org/2001/XMLSchema#nonNegativeInteger">1</owl:qualifiedCardinality>
                <owl:onClass rdf:resource="http://www.w3id.com/whow/onto/weather-monitoring/WeatherFeatureOfInterest"/>
            </owl:Restriction>
        </rdfs:subClassOf>
        <rdfs:subClassOf>
            <owl:Restriction>
                <owl:onProperty rdf:resource="https://w3id.org/italia/env/onto/inspire-mf/isObservationMadeBySensor"/>
                <owl:qualifiedCardinality rdf:datatype="http://www.w3.org/2001/XMLSchema#nonNegativeInteger">1</owl:qualifiedCardinality>
                <owl:onClass rdf:resource="http://www.w3id.com/whow/onto/weather-monitoring/WeatherSensor"/>
            </owl:Restriction>
        </rdfs:subClassOf>
        <rdfs:comment xml:lang="en">A specific type of observation obtained in the context of meteorogical measurements.</rdfs:comment>
        <rdfs:comment xml:lang="it">Una specifica osservazione fatta nel contesto delle rilevazioni meteorologiche.</rdfs:comment>
        <rdfs:isDefinedBy rdf:resource="http://www.w3id.com/whow/onto/weather-monitoring"/>
        <rdfs:label xml:lang="it">Osservazione Meteo</rdfs:label>
        <rdfs:label xml:lang="en">Weather Observation</rdfs:label>
        <owl:versionInfo xml:lang="it">stabile</owl:versionInfo>
        <owl:versionInfo xml:lang="en">stable</owl:versionInfo>
    </owl:Class>
    


    <!-- http://www.w3id.com/whow/onto/weather-monitoring/WeatherSensor -->

    <owl:Class rdf:about="http://www.w3id.com/whow/onto/weather-monitoring/WeatherSensor">
        <rdfs:subClassOf rdf:resource="https://w3id.org/italia/env/onto/inspire-mf/Sensor"/>
        <rdfs:subClassOf>
            <owl:Restriction>
                <owl:onProperty rdf:resource="https://w3id.org/italia/env/onto/inspire-mf/isHostedBy"/>
                <owl:allValuesFrom rdf:resource="http://www.w3id.com/whow/onto/weather-monitoring/WeatherStation"/>
            </owl:Restriction>
        </rdfs:subClassOf>
        <rdfs:subClassOf>
            <owl:Restriction>
                <owl:onProperty rdf:resource="http://www.w3id.com/whow/onto/weather-monitoring/hasValidityPeriod"/>
                <owl:maxQualifiedCardinality rdf:datatype="http://www.w3.org/2001/XMLSchema#nonNegativeInteger">1</owl:maxQualifiedCardinality>
                <owl:onClass rdf:resource="https://w3id.org/italia/env/onto/top/TimeInterval"/>
            </owl:Restriction>
        </rdfs:subClassOf>
        <rdfs:subClassOf>
            <owl:Restriction>
                <owl:onProperty rdf:resource="https://w3id.org/italia/env/onto/inspire-mf/hasSensorType"/>
                <owl:maxQualifiedCardinality rdf:datatype="http://www.w3.org/2001/XMLSchema#nonNegativeInteger">1</owl:maxQualifiedCardinality>
                <owl:onClass rdf:resource="http://www.w3id.com/whow/onto/weather-monitoring/WeatherSensorType"/>
            </owl:Restriction>
        </rdfs:subClassOf>
        <rdfs:comment xml:lang="it">La classe dei sensori meteo utilizzati per le rilevazioni meteorologiche.</rdfs:comment>
        <rdfs:comment xml:lang="en">The class of the weather sensor used to detect specific weather property.</rdfs:comment>
        <rdfs:isDefinedBy rdf:resource="http://www.w3id.com/whow/onto/weather-monitoring"/>
        <rdfs:label xml:lang="it">Sensore Meteo</rdfs:label>
        <rdfs:label xml:lang="en">Weather Sensor</rdfs:label>
        <owl:versionInfo xml:lang="it">stabile</owl:versionInfo>
        <owl:versionInfo xml:lang="en">stable</owl:versionInfo>
    </owl:Class>
    


    <!-- http://www.w3id.com/whow/onto/weather-monitoring/WeatherSensorType -->

    <owl:Class rdf:about="http://www.w3id.com/whow/onto/weather-monitoring/WeatherSensorType">
        <rdfs:subClassOf rdf:resource="https://w3id.org/italia/env/onto/top/Concept"/>
        <rdfs:comment xml:lang="it">La classe dei tipi di sensori meteo. Per esempio: termometro, pluviometro ecc.</rdfs:comment>
        <rdfs:comment xml:lang="en">The class of the various types of weather sensor. For instance: pluviometer , thermometer etc.</rdfs:comment>
        <rdfs:isDefinedBy rdf:resource="http://www.w3id.com/whow/onto/weather-monitoring"/>
        <rdfs:label xml:lang="it">Tipo di Sensore Meteo</rdfs:label>
        <rdfs:label xml:lang="en">Weather Sensor Type</rdfs:label>
        <owl:versionInfo xml:lang="it">stabile</owl:versionInfo>
        <owl:versionInfo xml:lang="en">stable</owl:versionInfo>
    </owl:Class>
    


    <!-- http://www.w3id.com/whow/onto/weather-monitoring/WeatherStation -->

    <owl:Class rdf:about="http://www.w3id.com/whow/onto/weather-monitoring/WeatherStation">
        <rdfs:subClassOf rdf:resource="https://w3id.org/italia/env/onto/inspire-mf/Platform"/>
        <rdfs:subClassOf>
            <owl:Restriction>
                <owl:onProperty rdf:resource="https://w3id.org/italia/env/onto/place/hasGeometry"/>
                <owl:qualifiedCardinality rdf:datatype="http://www.w3.org/2001/XMLSchema#nonNegativeInteger">1</owl:qualifiedCardinality>
                <owl:onClass rdf:resource="https://w3id.org/italia/env/onto/place/Geometry"/>
            </owl:Restriction>
        </rdfs:subClassOf>
        <rdfs:comment xml:lang="en">A specific type of platform hosting also different sensors that are used to detect weather conditions.</rdfs:comment>
        <rdfs:comment xml:lang="it">Una specifica piattaforma che ospita sensori per le rilevazioni meteorologiche.</rdfs:comment>
        <rdfs:isDefinedBy rdf:resource="http://www.w3id.com/whow/onto/weather-monitoring"/>
        <rdfs:label xml:lang="it">Stazione Meteo</rdfs:label>
        <rdfs:label xml:lang="en">Weather Station</rdfs:label>
        <owl:versionInfo xml:lang="it">stabile</owl:versionInfo>
        <owl:versionInfo xml:lang="en">stable</owl:versionInfo>
    </owl:Class>
    


    <!-- https://w3id.org/italia/env/onto/inspire-mf/FeatureOfInterest -->

    <owl:Class rdf:about="https://w3id.org/italia/env/onto/inspire-mf/FeatureOfInterest"/>
    


    <!-- https://w3id.org/italia/env/onto/inspire-mf/Observation -->

    <owl:Class rdf:about="https://w3id.org/italia/env/onto/inspire-mf/Observation"/>
    


    <!-- https://w3id.org/italia/env/onto/inspire-mf/ObservationParameter -->

    <owl:Class rdf:about="https://w3id.org/italia/env/onto/inspire-mf/ObservationParameter"/>
    


    <!-- https://w3id.org/italia/env/onto/inspire-mf/Platform -->

    <owl:Class rdf:about="https://w3id.org/italia/env/onto/inspire-mf/Platform"/>
    


    <!-- https://w3id.org/italia/env/onto/inspire-mf/Sensor -->

    <owl:Class rdf:about="https://w3id.org/italia/env/onto/inspire-mf/Sensor"/>
    


    <!-- https://w3id.org/italia/env/onto/place/Geometry -->

    <owl:Class rdf:about="https://w3id.org/italia/env/onto/place/Geometry"/>
    


    <!-- https://w3id.org/italia/env/onto/top/Concept -->

    <owl:Class rdf:about="https://w3id.org/italia/env/onto/top/Concept"/>
    


    <!-- https://w3id.org/italia/env/onto/top/TimeInterval -->

    <owl:Class rdf:about="https://w3id.org/italia/env/onto/top/TimeInterval"/>
    


    <!-- https://w3id.orgitalia/onto/TI/TimeInstant -->

    <owl:Class rdf:about="https://w3id.orgitalia/onto/TI/TimeInstant"/>
    


    <!-- 
    ///////////////////////////////////////////////////////////////////////////////////////
    //
    // Individuals
    //
    ///////////////////////////////////////////////////////////////////////////////////////
     -->

    


    <!-- http://www.w3id.com/whow/onto/weather-monitoring/Air -->

    <owl:NamedIndividual rdf:about="http://www.w3id.com/whow/onto/weather-monitoring/Air">
        <rdf:type rdf:resource="http://www.w3id.com/whow/onto/weather-monitoring/WeatherFeatureOfInterest"/>
        <rdfs:isDefinedBy rdf:resource="http://www.w3id.com/whow/onto/weather-monitoring"/>
        <rdfs:label xml:lang="en">Air</rdfs:label>
        <rdfs:label xml:lang="it">Aria</rdfs:label>
        <owl:versionInfo xml:lang="it">provvisoria</owl:versionInfo>
        <owl:versionInfo xml:lang="en">unstable</owl:versionInfo>
    </owl:NamedIndividual>
    


    <!-- http://www.w3id.com/whow/onto/weather-monitoring/GroundLevelSoil -->

    <owl:NamedIndividual rdf:about="http://www.w3id.com/whow/onto/weather-monitoring/GroundLevelSoil">
        <rdf:type rdf:resource="http://www.w3id.com/whow/onto/weather-monitoring/WeatherFeatureOfInterest"/>
        <rdfs:isDefinedBy rdf:resource="http://www.w3id.com/whow/onto/weather-monitoring"/>
        <rdfs:label xml:lang="it">All&apos;altezza del suolo</rdfs:label>
        <rdfs:label xml:lang="en">Ground Level Soil</rdfs:label>
        <owl:versionInfo xml:lang="it">provvisoria</owl:versionInfo>
        <owl:versionInfo xml:lang="en">unstable</owl:versionInfo>
    </owl:NamedIndividual>
    


    <!-- http://www.w3id.com/whow/onto/weather-monitoring/Rainfall -->

    <owl:NamedIndividual rdf:about="http://www.w3id.com/whow/onto/weather-monitoring/Rainfall">
        <rdf:type rdf:resource="http://www.w3id.com/whow/onto/weather-monitoring/WeatherFeatureOfInterest"/>
        <rdfs:isDefinedBy rdf:resource="http://www.w3id.com/whow/onto/weather-monitoring"/>
        <rdfs:label xml:lang="it">Pioggia</rdfs:label>
        <rdfs:label xml:lang="en">Rainfall</rdfs:label>
        <owl:versionInfo xml:lang="it">provvisoria</owl:versionInfo>
        <owl:versionInfo xml:lang="en">unstable</owl:versionInfo>
    </owl:NamedIndividual>
    


    <!-- http://www.w3id.com/whow/onto/weather-monitoring/Snow -->

    <owl:NamedIndividual rdf:about="http://www.w3id.com/whow/onto/weather-monitoring/Snow">
        <rdf:type rdf:resource="http://www.w3id.com/whow/onto/weather-monitoring/WeatherFeatureOfInterest"/>
        <rdfs:isDefinedBy rdf:resource="http://www.w3id.com/whow/onto/weather-monitoring"/>
        <rdfs:label xml:lang="it">Neve</rdfs:label>
        <rdfs:label xml:lang="en">Snow</rdfs:label>
        <owl:versionInfo xml:lang="it">provvisoria</owl:versionInfo>
        <owl:versionInfo xml:lang="en">unstable</owl:versionInfo>
    </owl:NamedIndividual>
    


    <!-- http://www.w3id.com/whow/onto/weather-monitoring/Wind -->

    <owl:NamedIndividual rdf:about="http://www.w3id.com/whow/onto/weather-monitoring/Wind">
        <rdf:type rdf:resource="http://www.w3id.com/whow/onto/weather-monitoring/WeatherFeatureOfInterest"/>
        <rdfs:isDefinedBy rdf:resource="http://www.w3id.com/whow/onto/weather-monitoring"/>
        <rdfs:label xml:lang="it">Vento</rdfs:label>
        <rdfs:label xml:lang="en">Wind</rdfs:label>
        <owl:versionInfo xml:lang="it">provvisoria</owl:versionInfo>
        <owl:versionInfo xml:lang="en">unstable</owl:versionInfo>
    </owl:NamedIndividual>
</rdf:RDF>



<!-- Generated by the OWL API (version 4.5.9.2019-02-01T07:24:44Z) https://github.com/owlcs/owlapi -->

