<?xml version="1.0"?>
<rdf:RDF xmlns="https://w3id.org/whow/onto/health-monitoring/"
     xml:base="https://w3id.org/whow/onto/health-monitoring/"
     xmlns:dc="http://purl.org/dc/elements/1.1/"
     xmlns:dct="http://purl.org/dc/terms/"
     xmlns:owl="http://www.w3.org/2002/07/owl#"
     xmlns:rdf="http://www.w3.org/1999/02/22-rdf-syntax-ns#"
     xmlns:xml="http://www.w3.org/XML/1998/namespace"
     xmlns:xsd="http://www.w3.org/2001/XMLSchema#"
     xmlns:rdfs="http://www.w3.org/2000/01/rdf-schema#">
    <owl:Ontology rdf:about="https://w3id.org/whow/onto/health-monitoring">
        <owl:versionIRI rdf:resource="https//w3id.org/whow/onto/health-monitoring/0.3"/>
        <owl:imports rdf:resource="https://w3id.org/italia/env/onto/top"/>
        <dc:description rdf:resource="https://raw.githubusercontent.com/whow-project/semantic-assets/main/ontologies/graphical-representation-ontologies/health-monitoring.png"/>
        <dct:description xml:lang="it">Questa è l&apos;ontologia del progetto WHOW utilizzata per rappresentare un insieme di indicatori utilizzati nel settore sanitario della regione Lombardia per monitorare alcuni parametri sanitari (ad esempio, la diffusione di malattie infettive, la distribuzione di farmaci, l&apos;andamento delle cause di morte e l&apos;accesso a specifiche strutture di ricovero). L&apos;ontologia è generale per modellare indicatori in ambito sanitario e non è strettamente dipendente dai dataset (aperti) della regione Lombardia.</dct:description>
        <dct:description xml:lang="en">This is the ontology of the WHOW project that used to represent a set of indicators used in the health sector of Lombardy region to monitor some health parameters (e.g., spread of infectious diseases, distribution of drugs, causes of deaths and access to specific inpatient facilities). The ontology is general to model indicators in the health domain and not strictly dependent on Lombarday region (open) datasets.</dct:description>
        <dct:issued rdf:datatype="http://www.w3.org/2001/XMLSchema#date">2022-10-03</dct:issued>
        <dct:modified rdf:datatype="http://www.w3.org/2001/XMLSchema#date">2023-06-05</dct:modified>
        <dct:title xml:lang="en">Health Care Indicator Monitoring Ontology</dct:title>
        <dct:title xml:lang="it">Ontologia di Monitoraggio di Indicatori della Salute</dct:title>
        <rdfs:label xml:lang="en">Health Care Indicator Monitoring Ontology</rdfs:label>
        <rdfs:label xml:lang="it">Ontologia di Monitoraggio di Indicatori della Salute</rdfs:label>
        <owl:versionInfo xml:lang="en">Version 0.3 - June 2023 - modified some elements of the ontology (introduction of the property hasScope for the Cohort and related elements, revision of the organisations involved in the computation of some indicators)</owl:versionInfo>
    </owl:Ontology>



    <!--
    ///////////////////////////////////////////////////////////////////////////////////////
    //
    // Annotation properties
    //
    ///////////////////////////////////////////////////////////////////////////////////////
     -->




    <!-- http://purl.org/dc/elements/1.1/description -->

    <owl:AnnotationProperty rdf:about="http://purl.org/dc/elements/1.1/description"/>



    <!-- http://purl.org/dc/terms/description -->

    <owl:AnnotationProperty rdf:about="http://purl.org/dc/terms/description"/>



    <!-- http://purl.org/dc/terms/issued -->

    <owl:AnnotationProperty rdf:about="http://purl.org/dc/terms/issued"/>



    <!-- http://purl.org/dc/terms/modified -->

    <owl:AnnotationProperty rdf:about="http://purl.org/dc/terms/modified"/>



    <!-- http://purl.org/dc/terms/title -->

    <owl:AnnotationProperty rdf:about="http://purl.org/dc/terms/title"/>



    <!--
    ///////////////////////////////////////////////////////////////////////////////////////
    //
    // Object Properties
    //
    ///////////////////////////////////////////////////////////////////////////////////////
     -->




    <!-- https://w3id.org/italia/env/onto/inspire-mf/isIndicatorOf -->

    <owl:ObjectProperty rdf:about="https://w3id.org/italia/env/onto/inspire-mf/isIndicatorOf"/>



    <!-- https://w3id.org/italia/env/onto/top/isClassifiedBy -->

    <owl:ObjectProperty rdf:about="https://w3id.org/italia/env/onto/top/isClassifiedBy"/>



    <!-- https://w3id.org/whow/onto/health-monitoring/affectedBy -->

    <owl:ObjectProperty rdf:about="https://w3id.org/whow/onto/health-monitoring/affectedBy">
        <rdfs:subPropertyOf rdf:resource="https://w3id.org/whow/onto/health-monitoring/hasScope"/>
        <rdfs:domain rdf:resource="https://w3id.org/whow/onto/health-monitoring/ClinicalCohort"/>
        <rdfs:range rdf:resource="https://w3id.org/whow/onto/health-monitoring/Disease"/>
        <rdfs:comment xml:lang="en">Property that links the clinical cohort with the disease they are affected by.</rdfs:comment>
        <rdfs:comment xml:lang="it">Proprietà che consente di collegare la coorte clinica con la malattia  di cui sono affetti.</rdfs:comment>
        <rdfs:isDefinedBy rdf:resource="https://w3id.org/whow/onto/health-monitoring"/>
        <rdfs:label xml:lang="en">affected by</rdfs:label>
        <rdfs:label xml:lang="it">affetta da</rdfs:label>
        <owl:versionInfo xml:lang="it">provvisoria</owl:versionInfo>
        <owl:versionInfo xml:lang="en">unstable</owl:versionInfo>
    </owl:ObjectProperty>



    <!-- https://w3id.org/whow/onto/health-monitoring/assumed -->

    <owl:ObjectProperty rdf:about="https://w3id.org/whow/onto/health-monitoring/assumed">
        <rdfs:subPropertyOf rdf:resource="https://w3id.org/whow/onto/health-monitoring/hasScope"/>
        <rdfs:domain rdf:resource="https://w3id.org/whow/onto/health-monitoring/ClinicalCohort"/>
        <rdfs:range rdf:resource="https://w3id.org/whow/onto/health-monitoring/DrugType"/>
        <rdfs:comment xml:lang="en">Property that specialises has scope, used to define the clinical cohort that assumed specific types of drugs, when the indicator to be calculated concerns the drug distribution rate.</rdfs:comment>
        <rdfs:comment xml:lang="it">Proprietà che specializza la proprietà ha ambito usata per definire la coorte clinica che ha assunto specifiche tipologie di farmaci, quando l&apos;indicatore da calcolare riguarda il tasso di distribuzione di farmaci.</rdfs:comment>
        <rdfs:isDefinedBy rdf:resource="https://w3id.org/whow/onto/health-monitoring"/>
        <rdfs:label xml:lang="en">assumed</rdfs:label>
        <rdfs:label xml:lang="it">assunto</rdfs:label>
        <owl:versionInfo xml:lang="it">provvisoria</owl:versionInfo>
        <owl:versionInfo xml:lang="en">unstable</owl:versionInfo>
    </owl:ObjectProperty>



    <!-- https://w3id.org/whow/onto/health-monitoring/diedFrom -->

    <owl:ObjectProperty rdf:about="https://w3id.org/whow/onto/health-monitoring/diedFrom">
        <rdfs:subPropertyOf rdf:resource="https://w3id.org/whow/onto/health-monitoring/hasScope"/>
        <rdfs:domain rdf:resource="https://w3id.org/whow/onto/health-monitoring/ClinicalCohort"/>
        <rdfs:range rdf:resource="https://w3id.org/whow/onto/health-monitoring/CauseOfDeath"/>
        <rdfs:comment xml:lang="en">Property that specialises the has scope properties in order to define the clinical cohort died from causes of death when the indicator to be computed is about  the number of deaths from specific causes of death.</rdfs:comment>
        <rdfs:comment xml:lang="it">Proprietà che specializza la proprietà ha ambito usata per definire la coorte clinica deceduta per  specifiche cause di morte, quando l&apos;indicatore da calcolare riguarda il numero dei decessi per specifiche cause di morte.</rdfs:comment>
        <rdfs:isDefinedBy rdf:resource="https://w3id.org/whow/onto/health-monitoring"/>
        <rdfs:label xml:lang="en">died from</rdfs:label>
        <rdfs:label xml:lang="it">morte per</rdfs:label>
        <owl:versionInfo xml:lang="it">provvisoria</owl:versionInfo>
        <owl:versionInfo xml:lang="en">unstable</owl:versionInfo>
    </owl:ObjectProperty>



    <!-- https://w3id.org/whow/onto/health-monitoring/doneForHCIndicator -->

    <owl:ObjectProperty rdf:about="https://w3id.org/whow/onto/health-monitoring/doneForHCIndicator">
        <rdfs:domain rdf:resource="https://w3id.org/whow/onto/health-monitoring/HealthcareIndicatorCalculation"/>
        <rdfs:range rdf:resource="https://w3id.org/whow/onto/health-monitoring/HealthcareIndicator"/>
        <rdfs:comment xml:lang="en">Property that links the calculation of an indicator with the healthcare indicator itself.</rdfs:comment>
        <rdfs:comment xml:lang="it">Proprietà che collega il calcolo dell&apos;indicatore, con l&apos;indicatore stesso.</rdfs:comment>
        <rdfs:label xml:lang="en">done for healthcare indicator</rdfs:label>
        <rdfs:label xml:lang="it">fatto per indicatore sanitario</rdfs:label>
        <owl:versionInfo xml:lang="it">stabile</owl:versionInfo>
        <owl:versionInfo xml:lang="en">stable</owl:versionInfo>
    </owl:ObjectProperty>



    <!-- https://w3id.org/whow/onto/health-monitoring/hasCohortCriteriaDescription -->

    <owl:ObjectProperty rdf:about="https://w3id.org/whow/onto/health-monitoring/hasCohortCriteriaDescription">
        <rdfs:domain rdf:resource="https://w3id.org/whow/onto/health-monitoring/ClinicalCohort"/>
        <rdfs:range rdf:resource="https://w3id.org/whow/onto/health-monitoring/CohortCriteriaDescription"/>
        <rdfs:comment xml:lang="en">Property that links the clinical cohort with the description of the criteria that determine the dimension of the cohort.</rdfs:comment>
        <rdfs:comment xml:lang="it">Proprietà che lega la coorte clinica con la descrizioni dei criteri che ne determinano la sua dimensione.</rdfs:comment>
        <rdfs:isDefinedBy rdf:resource="https://w3id.org/whow/onto/health-monitoring"/>
        <rdfs:label xml:lang="it">ha descrizione criteri coorte clinica</rdfs:label>
        <rdfs:label xml:lang="en">has clinical cohort criteria description</rdfs:label>
        <owl:versionInfo xml:lang="it">stabile</owl:versionInfo>
        <owl:versionInfo xml:lang="en">stable</owl:versionInfo>
    </owl:ObjectProperty>



    <!-- https://w3id.org/whow/onto/health-monitoring/hasCriterion -->

    <owl:ObjectProperty rdf:about="https://w3id.org/whow/onto/health-monitoring/hasCriterion">
        <rdfs:domain rdf:resource="https://w3id.org/whow/onto/health-monitoring/CohortCriteriaDescription"/>
        <rdfs:range rdf:resource="https://w3id.org/whow/onto/health-monitoring/Criterion"/>
        <rdfs:comment xml:lang="en">Property that links the description of the criteria for the dimension of the clinical cohort to each single criterion.</rdfs:comment>
        <rdfs:comment xml:lang="it">Proprietà che collega la descrizione dei criteri per la dimensione della coorte clinica a ogni singolo criterio.</rdfs:comment>
        <rdfs:isDefinedBy rdf:resource="https://w3id.org/whow/onto/health-monitoring"/>
        <rdfs:label xml:lang="it">ha criterio</rdfs:label>
        <rdfs:label xml:lang="en">has criterion</rdfs:label>
        <owl:versionInfo xml:lang="it">stabile</owl:versionInfo>
        <owl:versionInfo xml:lang="en">stable</owl:versionInfo>
    </owl:ObjectProperty>



    <!-- https://w3id.org/whow/onto/health-monitoring/hasHealthcareIndicatorValue -->

    <owl:ObjectProperty rdf:about="https://w3id.org/whow/onto/health-monitoring/hasHealthcareIndicatorValue">
        <rdfs:domain rdf:resource="https://w3id.org/whow/onto/health-monitoring/HealthcareIndicatorCalculation"/>
        <rdfs:range rdf:resource="https://w3id.org/italia/env/onto/top/Value"/>
        <rdfs:comment xml:lang="en">Property used to link the healthcare indicator calculation with the related value.</rdfs:comment>
        <rdfs:comment xml:lang="it">Proprietà utilizzata per collegare il calcolo dell&apos;indicatore di salute con il relativo valore.</rdfs:comment>
        <rdfs:isDefinedBy rdf:resource="https://w3id.org/whow/onto/health-monitoring"/>
        <rdfs:label xml:lang="it">ha valore indicatore di salute</rdfs:label>
        <rdfs:label xml:lang="en">has healthcare indicator value</rdfs:label>
        <owl:versionInfo xml:lang="it">stabile</owl:versionInfo>
        <owl:versionInfo xml:lang="en">stable</owl:versionInfo>
    </owl:ObjectProperty>



    <!-- https://w3id.org/whow/onto/health-monitoring/hasScope -->

    <owl:ObjectProperty rdf:about="https://w3id.org/whow/onto/health-monitoring/hasScope">
        <rdfs:domain rdf:resource="https://w3id.org/whow/onto/health-monitoring/ClinicalCohort"/>
        <rdfs:range rdf:resource="https://w3id.org/italia/env/onto/top/Concept"/>
        <rdfs:comment xml:lang="en">Generic property that links the cohort used in the indicator calculation to the context (e.g., disease, drug use, causes of deaths)</rdfs:comment>
        <rdfs:comment xml:lang="it">Proprietà generica che collega la coorte utilizzata nel calcolo dell&apos;indicatore un contesto (ad esempio, malattia di cui affetta, uso di droghe, cause per cui è morta).</rdfs:comment>
        <rdfs:isDefinedBy rdf:resource="https://w3id.org/whow/onto/health-monitoring"/>
        <rdfs:label xml:lang="it">ha ambito</rdfs:label>
        <rdfs:label xml:lang="en">has scope</rdfs:label>
        <owl:versionInfo xml:lang="it">stabile</owl:versionInfo>
        <owl:versionInfo xml:lang="en">stable</owl:versionInfo>
    </owl:ObjectProperty>



    <!-- https://w3id.org/whow/onto/health-monitoring/isResponsibleFor -->

    <owl:ObjectProperty rdf:about="https://w3id.org/whow/onto/health-monitoring/isResponsibleFor">
        <owl:inverseOf rdf:resource="https://w3id.org/whow/onto/health-monitoring/isUnderResponsibilityOf"/>
        <rdfs:domain rdf:resource="https://w3id.org/whow/onto/health-monitoring/HealthcareAuthority"/>
        <rdfs:range rdf:resource="https://w3id.org/italia/env/onto/top/Location"/>
        <rdfs:comment xml:lang="en">Property used to indicate the responsibility of a health organisation with respect to a certain territorial area. The jurisdiction of the health organisation.</rdfs:comment>
        <rdfs:comment xml:lang="it">Proprietà utilizzata per indicare la responsabilità di un&apos;organizzazione sanitaria rispetto a una certa area territoriale. La giurisdizione dell&apos;azienda sanitaria.</rdfs:comment>
        <rdfs:isDefinedBy rdf:resource="https://w3id.org/whow/onto/health-monitoring"/>
        <rdfs:label xml:lang="en">is responsible for</rdfs:label>
        <rdfs:label xml:lang="it">è responsabile di</rdfs:label>
        <owl:versionInfo xml:lang="it">stabile</owl:versionInfo>
        <owl:versionInfo xml:lang="en">stable</owl:versionInfo>
    </owl:ObjectProperty>



    <!-- https://w3id.org/whow/onto/health-monitoring/isTerritoriallyCompetentFor -->

    <owl:ObjectProperty rdf:about="https://w3id.org/whow/onto/health-monitoring/isTerritoriallyCompetentFor">
        <rdfs:domain rdf:resource="https://w3id.org/whow/onto/health-monitoring/HealthcareAuthority"/>
        <rdfs:range rdf:resource="https://w3id.org/whow/onto/health-monitoring/InpatientFacility"/>
        <rdfs:comment xml:lang="en">Property that connects the typically local health authority with the relevant inpatient facilities.</rdfs:comment>
        <rdfs:comment xml:lang="it">Proprietà che collega l&apos;autorità competente in materia sanitaria, tipicamente locale, con le relative strutture di ricovero di pertinenza.</rdfs:comment>
        <rdfs:isDefinedBy rdf:resource="https://w3id.org/whow/onto/health-monitoring"/>
        <rdfs:label xml:lang="en">is territorial competent for</rdfs:label>
        <rdfs:label xml:lang="it">è territorialmente competente per</rdfs:label>
        <owl:versionInfo xml:lang="it">stabile</owl:versionInfo>
        <owl:versionInfo xml:lang="en">stable</owl:versionInfo>
    </owl:ObjectProperty>



    <!-- https://w3id.org/whow/onto/health-monitoring/isUnderResponsibilityOf -->

    <owl:ObjectProperty rdf:about="https://w3id.org/whow/onto/health-monitoring/isUnderResponsibilityOf">
        <rdfs:domain rdf:resource="https://w3id.org/italia/env/onto/top/Location"/>
        <rdfs:range rdf:resource="https://w3id.org/whow/onto/health-monitoring/HealthcareAuthority"/>
        <rdfs:comment xml:lang="en">Property used to link the geographical area which is of competence of a specific healthcare authority.</rdfs:comment>
        <rdfs:comment xml:lang="it">Proprietà utilizzata per collegare un&apos;area geografica a l&apos;autorità sanitaria di competenza di quell&apos;area.</rdfs:comment>
        <rdfs:isDefinedBy rdf:resource="https://w3id.org/whow/onto/health-monitoring"/>
        <rdfs:label xml:lang="en">is under responsiblity of</rdfs:label>
        <rdfs:label xml:lang="it">è sotto la responsabilità di</rdfs:label>
        <owl:versionInfo xml:lang="it">stabile</owl:versionInfo>
        <owl:versionInfo xml:lang="en">stable</owl:versionInfo>
    </owl:ObjectProperty>



    <!-- https://w3id.org/whow/onto/health-monitoring/narrower -->

    <owl:ObjectProperty rdf:about="https://w3id.org/whow/onto/health-monitoring/narrower">
        <rdfs:domain rdf:resource="https://w3id.org/whow/onto/health-monitoring/DiseaseType"/>
        <rdfs:range rdf:resource="https://w3id.org/whow/onto/health-monitoring/DiseaseType"/>
        <rdfs:comment xml:lang="en">Property used to create a taxonomy of different types of diseases.</rdfs:comment>
        <rdfs:comment xml:lang="it">Proprietà che consente di modellare una tassonomia di tipi di malattie.</rdfs:comment>
        <rdfs:isDefinedBy rdf:resource="https://w3id.org/whow/onto/health-monitoring"/>
        <rdfs:label xml:lang="en">narrower</rdfs:label>
        <rdfs:label xml:lang="it">sotto insieme</rdfs:label>
        <owl:versionInfo xml:lang="it">stabile</owl:versionInfo>
        <owl:versionInfo xml:lang="en">stable</owl:versionInfo>
    </owl:ObjectProperty>



    <!-- https://w3id.org/whow/onto/health-monitoring/ofClinicalCohort -->

    <owl:ObjectProperty rdf:about="https://w3id.org/whow/onto/health-monitoring/ofClinicalCohort">
        <rdfs:subPropertyOf rdf:resource="http://www.w3.org/2002/07/owl#topObjectProperty"/>
        <rdfs:domain rdf:resource="https://w3id.org/whow/onto/health-monitoring/HealthcareIndicatorCalculation"/>
        <rdfs:range rdf:resource="https://w3id.org/whow/onto/health-monitoring/ClinicalCohort"/>
        <rdfs:comment xml:lang="en">Property used to specify the clinical cohort for the healthcare indicator calculation.</rdfs:comment>
        <rdfs:comment xml:lang="it">Proprietà utilizzata per indicare la coorte clinica considerata nel calcolo dell&apos;indicatore di salute.</rdfs:comment>
        <rdfs:isDefinedBy rdf:resource="https://w3id.org/whow/onto/health-monitoring"/>
        <rdfs:label xml:lang="it">di coorte clinica</rdfs:label>
        <rdfs:label xml:lang="en">of clinical cohort</rdfs:label>
        <owl:versionInfo xml:lang="it">stabile</owl:versionInfo>
        <owl:versionInfo xml:lang="en">stable</owl:versionInfo>
    </owl:ObjectProperty>



    <!-- https://w3id.org/whow/onto/health-monitoring/subIndicator -->

    <owl:ObjectProperty rdf:about="https://w3id.org/whow/onto/health-monitoring/subIndicator">
        <rdfs:domain rdf:resource="https://w3id.org/whow/onto/health-monitoring/HealthcareIndicatorCalculation"/>
        <rdfs:range rdf:resource="https://w3id.org/whow/onto/health-monitoring/HealthcareIndicatorCalculation"/>
        <rdfs:comment xml:lang="en">Property used to create a taxonomy of the calculation of healthcare indicators.</rdfs:comment>
        <rdfs:comment xml:lang="it">Proprietà utilizzata per creare tassonomie dei calcoli degli indicatori di salute. Utile quando alcuni calcoli dipendono da altri.</rdfs:comment>
        <rdfs:isDefinedBy rdf:resource="https://w3id.org/whow/onto/health-monitoring"/>
        <rdfs:label xml:lang="it">sotto indicatore</rdfs:label>
        <rdfs:label xml:lang="en">sub indicator</rdfs:label>
        <owl:versionInfo xml:lang="it">stabile</owl:versionInfo>
        <owl:versionInfo xml:lang="en">stable</owl:versionInfo>
    </owl:ObjectProperty>



    <!--
    ///////////////////////////////////////////////////////////////////////////////////////
    //
    // Data properties
    //
    ///////////////////////////////////////////////////////////////////////////////////////
     -->




    <!-- https://w3id.org/whow/onto/health-monitoring/totalValue -->

    <owl:DatatypeProperty rdf:about="https://w3id.org/whow/onto/health-monitoring/totalValue">
        <rdfs:domain rdf:resource="https://w3id.org/whow/onto/health-monitoring/Population"/>
        <rdfs:range rdf:resource="http://www.w3.org/2001/XMLSchema#float"/>
        <rdfs:comment xml:lang="en">Property that indicates the total popolation of a certain area of reference.</rdfs:comment>
        <rdfs:comment xml:lang="it">Proprietà che indica il valore totale della popolazione in una certa area di riferimento.</rdfs:comment>
        <rdfs:isDefinedBy rdf:resource="https://w3id.org/whow/onto/health-monitoring"/>
        <rdfs:label xml:lang="en">total value</rdfs:label>
        <rdfs:label xml:lang="it">valore totale</rdfs:label>
        <owl:versionInfo xml:lang="it">stabile</owl:versionInfo>
        <owl:versionInfo xml:lang="en">stable</owl:versionInfo>
    </owl:DatatypeProperty>



    <!--
    ///////////////////////////////////////////////////////////////////////////////////////
    //
    // Classes
    //
    ///////////////////////////////////////////////////////////////////////////////////////
     -->




    <!-- https://w3id.org/italia/env/onto/inspire-mf/Indicator -->

    <owl:Class rdf:about="https://w3id.org/italia/env/onto/inspire-mf/Indicator"/>



    <!-- https://w3id.org/italia/env/onto/top/Characteristic -->

    <owl:Class rdf:about="https://w3id.org/italia/env/onto/top/Characteristic"/>



    <!-- https://w3id.org/italia/env/onto/top/Concept -->

    <owl:Class rdf:about="https://w3id.org/italia/env/onto/top/Concept"/>



    <!-- https://w3id.org/italia/env/onto/top/Description -->

    <owl:Class rdf:about="https://w3id.org/italia/env/onto/top/Description"/>



    <!-- https://w3id.org/italia/env/onto/top/Entity -->

    <owl:Class rdf:about="https://w3id.org/italia/env/onto/top/Entity"/>



    <!-- https://w3id.org/italia/env/onto/top/Eventuality -->

    <owl:Class rdf:about="https://w3id.org/italia/env/onto/top/Eventuality"/>



    <!-- https://w3id.org/italia/env/onto/top/Location -->

    <owl:Class rdf:about="https://w3id.org/italia/env/onto/top/Location"/>



    <!-- https://w3id.org/italia/env/onto/top/Organisation -->

    <owl:Class rdf:about="https://w3id.org/italia/env/onto/top/Organisation"/>



    <!-- https://w3id.org/italia/env/onto/top/Value -->

    <owl:Class rdf:about="https://w3id.org/italia/env/onto/top/Value"/>



    <!-- https://w3id.org/whow/onto/health-monitoring/CauseOfDeath -->

    <owl:Class rdf:about="https://w3id.org/whow/onto/health-monitoring/CauseOfDeath">
        <rdfs:subClassOf rdf:resource="https://w3id.org/italia/env/onto/top/Concept"/>
        <rdfs:subClassOf>
            <owl:Restriction>
                <owl:onProperty rdf:resource="https://w3id.org/italia/env/onto/top/isClassifiedBy"/>
                <owl:allValuesFrom rdf:resource="https://w3id.org/whow/onto/health-monitoring/GroupCauseOfDeath"/>
            </owl:Restriction>
        </rdfs:subClassOf>
        <rdfs:comment xml:lang="it">La classe di tutte quelle circostanze/situazioni/condizioni morbose che portano direttamente alla morte della persona.</rdfs:comment>
        <rdfs:comment xml:lang="en">The class of all those circumstances/situations/pathological conditions that lead directly to a person&apos;s death.</rdfs:comment>
        <rdfs:isDefinedBy rdf:resource="https://w3id.org/whow/onto/health-monitoring"/>
        <rdfs:label xml:lang="it">Causa di Morte</rdfs:label>
        <rdfs:label xml:lang="en">Cause of Death</rdfs:label>
        <owl:versionInfo xml:lang="it">provvisoria</owl:versionInfo>
        <owl:versionInfo xml:lang="en">unstable</owl:versionInfo>
    </owl:Class>



    <!-- https://w3id.org/whow/onto/health-monitoring/ClinicalCohort -->

    <owl:Class rdf:about="https://w3id.org/whow/onto/health-monitoring/ClinicalCohort">
        <rdfs:subClassOf rdf:resource="https://w3id.org/whow/onto/health-monitoring/Population"/>
        <rdfs:subClassOf>
            <owl:Restriction>
                <owl:onProperty rdf:resource="https://w3id.org/whow/onto/health-monitoring/hasScope"/>
                <owl:allValuesFrom rdf:resource="https://w3id.org/italia/env/onto/top/Concept"/>
            </owl:Restriction>
        </rdfs:subClassOf>
        <rdfs:comment xml:lang="it">L&apos;insieme della sola popolazione clinica (è infatti sotto classe della popolazione generale) che rappresenta la popolazione su cui si calcola l&apos;indicatore di salute. Essa è caratterizzata da criteri o parametri per la sua composizione (e.g., sesso, età) ed è associata a un generico ambito che varia a seconda del tipo di indicatore che viene calcolato.</rdfs:comment>
        <rdfs:comment xml:lang="en">The class of the sole clinical cohort (actually a subclass of the general population) on which the health indicator is calculated. It is characterised by criteria or parameters for its composition (e.g. gender, age) and is associated with a generic scope that varies according to the type of indicator being calculated.</rdfs:comment>
        <rdfs:isDefinedBy rdf:resource="https://w3id.org/whow/onto/health-monitoring"/>
        <rdfs:label xml:lang="en">Clinical Cohort</rdfs:label>
        <rdfs:label xml:lang="it">Coorte Clinica</rdfs:label>
        <owl:versionInfo xml:lang="it">stabile</owl:versionInfo>
        <owl:versionInfo xml:lang="en">stable</owl:versionInfo>
    </owl:Class>



    <!-- https://w3id.org/whow/onto/health-monitoring/CohortCriteriaDescription -->

    <owl:Class rdf:about="https://w3id.org/whow/onto/health-monitoring/CohortCriteriaDescription">
        <rdfs:subClassOf rdf:resource="https://w3id.org/italia/env/onto/top/Description"/>
        <rdfs:subClassOf>
            <owl:Restriction>
                <owl:onProperty rdf:resource="https://w3id.org/whow/onto/health-monitoring/hasCriterion"/>
                <owl:someValuesFrom rdf:resource="https://w3id.org/whow/onto/health-monitoring/Criterion"/>
            </owl:Restriction>
        </rdfs:subClassOf>
        <rdfs:subClassOf>
            <owl:Restriction>
                <owl:onProperty rdf:resource="https://w3id.org/italia/env/onto/top/value"/>
                <owl:someValuesFrom rdf:resource="http://www.w3.org/2000/01/rdf-schema#Literal"/>
            </owl:Restriction>
        </rdfs:subClassOf>
        <rdfs:comment xml:lang="it">La classe rappresenta una reificazione e implementa il design pattern dell&apos;ontologia Description. Grazie a questo pattern è possibile descrivere  la dimensione della coorte clinica sulla base di criteri, non sempre noti a priori, e dei relativi valori.</rdfs:comment>
        <rdfs:comment xml:lang="en">The class represents a reification and implements the ontology design pattern named Description. With this pattern it is possible to describe the dimension of the clinical cohort on the basis of criteria, not always known a priori, and their values,</rdfs:comment>
        <rdfs:isDefinedBy rdf:resource="https://w3id.org/whow/onto/health-monitoring"/>
        <rdfs:label xml:lang="en">Cohort Criteria Description</rdfs:label>
        <rdfs:label xml:lang="it">Descrizione dei Criteri per Dimensione Popolazione Clinica</rdfs:label>
        <owl:versionInfo xml:lang="it">stabile</owl:versionInfo>
        <owl:versionInfo xml:lang="en">stable</owl:versionInfo>
    </owl:Class>



    <!-- https://w3id.org/whow/onto/health-monitoring/Criterion -->

    <owl:Class rdf:about="https://w3id.org/whow/onto/health-monitoring/Criterion">
        <rdfs:subClassOf rdf:resource="https://w3id.org/italia/env/onto/top/Characteristic"/>
        <rdfs:comment xml:lang="it">La classe che rappresenta criteri. Nello specifico contesto di questa ontologia sono i criteri attraverso cui viene descritta la dimensione della popolazione clinica che concorre al calcolo dell&apos;indicatore di salute. Esempi di criteri includono: età. sesso, anno di inizio sintomi per una malattia infettiva, ecc.</rdfs:comment>
        <rdfs:comment xml:lang="en">The class representing criteria. In the specific context of this ontology, these are the criteria by which the  dimension of the clinical population contributing to the calculation of the health indicator is described. Examples of criteria include: age. gender, year of start of symptoms for an infectious disease, etc.</rdfs:comment>
        <rdfs:isDefinedBy rdf:resource="https://w3id.org/whow/onto/health-monitoring"/>
        <rdfs:label xml:lang="it">Criterio</rdfs:label>
        <rdfs:label xml:lang="en">Criterion</rdfs:label>
        <owl:versionInfo xml:lang="it">stabile</owl:versionInfo>
        <owl:versionInfo xml:lang="en">stable</owl:versionInfo>
    </owl:Class>



    <!-- https://w3id.org/whow/onto/health-monitoring/Disease -->

    <owl:Class rdf:about="https://w3id.org/whow/onto/health-monitoring/Disease">
        <rdfs:subClassOf rdf:resource="https://w3id.org/italia/env/onto/top/Concept"/>
        <rdfs:comment xml:lang="it">La classe che rappresenta una malattia (e.g., COVID-19, la varicella, etc.)</rdfs:comment>
        <rdfs:comment xml:lang="en">The class that represents the disease (e.g., COVID-19).</rdfs:comment>
        <rdfs:isDefinedBy rdf:resource="https://w3id.org/whow/onto/health-monitoring"/>
        <rdfs:label xml:lang="en">Disease</rdfs:label>
        <rdfs:label xml:lang="it">Malattia</rdfs:label>
        <owl:versionInfo xml:lang="it">stabile</owl:versionInfo>
        <owl:versionInfo xml:lang="en">stable</owl:versionInfo>
    </owl:Class>



    <!-- https://w3id.org/whow/onto/health-monitoring/DiseaseType -->

    <owl:Class rdf:about="https://w3id.org/whow/onto/health-monitoring/DiseaseType">
        <rdfs:subClassOf rdf:resource="https://w3id.org/italia/env/onto/top/Characteristic"/>
        <rdfs:subClassOf rdf:resource="https://w3id.org/italia/env/onto/top/Concept"/>
        <rdfs:comment xml:lang="it">La classe dei tipi di malattia.</rdfs:comment>
        <rdfs:comment xml:lang="en">The class of the types of diseases</rdfs:comment>
        <rdfs:isDefinedBy rdf:resource="https://w3id.org/whow/onto/health-monitoring"/>
        <rdfs:label xml:lang="en">Disease Type</rdfs:label>
        <rdfs:label xml:lang="it">Tipo di Malattia</rdfs:label>
        <owl:versionInfo xml:lang="it">stabile</owl:versionInfo>
        <owl:versionInfo xml:lang="en">stable</owl:versionInfo>
    </owl:Class>



    <!-- https://w3id.org/whow/onto/health-monitoring/DrugDistributionIndicatorCalculation -->

    <owl:Class rdf:about="https://w3id.org/whow/onto/health-monitoring/DrugDistributionIndicatorCalculation">
        <rdfs:subClassOf rdf:resource="https://w3id.org/whow/onto/health-monitoring/HealthcareIndicatorCalculation"/>
        <rdfs:comment xml:lang="it">La classe del calcolo dell&apos;indicatore relativo alla distribuzione dei farmaci. Questa classe è equivalente al &apos;calcolo dell&apos;indicatore di salute quando l&apos;indicatore sanitario è  &apos;distribuzione farmaci&apos;.&apos;</rdfs:comment>
        <rdfs:comment xml:lang="en">The class of the drug distribution indicator calculation. This class is equivalent to the &apos;health indicator calculation when the health indicator is &apos;drug distribution&apos;.&apos;</rdfs:comment>
        <rdfs:isDefinedBy rdf:resource="https://w3id.org/whow/onto/health-monitoring"/>
        <rdfs:label xml:lang="it">Calcolo dell&apos;Indicatore Distribuzione Farmaci</rdfs:label>
        <rdfs:label xml:lang="en">Drug Distribution Indicator Calculation</rdfs:label>
        <owl:versionInfo xml:lang="it">provvisoria</owl:versionInfo>
        <owl:versionInfo xml:lang="en">unstable</owl:versionInfo>
    </owl:Class>



    <!-- https://w3id.org/whow/onto/health-monitoring/DrugType -->

    <owl:Class rdf:about="https://w3id.org/whow/onto/health-monitoring/DrugType">
        <rdfs:subClassOf rdf:resource="https://w3id.org/italia/env/onto/top/Concept"/>
        <rdfs:subClassOf>
            <owl:Restriction>
                <owl:onProperty rdf:resource="https://w3id.org/italia/env/onto/top/identifier"/>
                <owl:someValuesFrom rdf:resource="http://www.w3.org/2000/01/rdf-schema#Literal"/>
            </owl:Restriction>
        </rdfs:subClassOf>
        <rdfs:subClassOf>
            <owl:Restriction>
                <owl:onProperty rdf:resource="https://w3id.org/italia/env/onto/top/name"/>
                <owl:someValuesFrom rdf:resource="http://www.w3.org/1999/02/22-rdf-syntax-ns#PlainLiteral"/>
            </owl:Restriction>
        </rdfs:subClassOf>
        <rdfs:comment xml:lang="it">La classe delle tipologie di farmaci assunte da persone.</rdfs:comment>
        <rdfs:comment xml:lang="en">The class of categories of drugs consumed by people.</rdfs:comment>
        <rdfs:isDefinedBy rdf:resource="https://w3id.org/whow/onto/health-monitoring"/>
        <rdfs:label xml:lang="en">Drug Type</rdfs:label>
        <rdfs:label xml:lang="it">Tipo di Farmaco</rdfs:label>
        <owl:versionInfo xml:lang="it">provvisoria</owl:versionInfo>
        <owl:versionInfo xml:lang="en">unstable</owl:versionInfo>
    </owl:Class>



    <!-- https://w3id.org/whow/onto/health-monitoring/GroupCauseOfDeath -->

    <owl:Class rdf:about="https://w3id.org/whow/onto/health-monitoring/GroupCauseOfDeath">
        <rdfs:subClassOf rdf:resource="https://w3id.org/italia/env/onto/top/Concept"/>
        <rdfs:comment xml:lang="en">Classification consisting of macro-categories of causes leading to the death of people.</rdfs:comment>
        <rdfs:comment xml:lang="it">Classificazione formata da macro-categorie di cause che portano alla morte di persone.</rdfs:comment>
        <rdfs:isDefinedBy rdf:resource="https://w3id.org/whow/onto/health-monitoring"/>
        <rdfs:label xml:lang="en">Group pf Causes of Death</rdfs:label>
        <rdfs:label xml:lang="it">Gruppo di cause di morte</rdfs:label>
        <owl:versionInfo xml:lang="it">stabile</owl:versionInfo>
        <owl:versionInfo xml:lang="en">stable</owl:versionInfo>
    </owl:Class>



    <!-- https://w3id.org/whow/onto/health-monitoring/HealthConditionIndicatorCalculation -->

    <owl:Class rdf:about="https://w3id.org/whow/onto/health-monitoring/HealthConditionIndicatorCalculation">
        <rdfs:subClassOf rdf:resource="https://w3id.org/whow/onto/health-monitoring/HealthcareIndicatorCalculation"/>
        <rdfs:comment xml:lang="it">La classe del calcolo dell&apos;indicatore relativo alle condizioni generali di salute della popolazione. Questa classe è equivalente al &apos;calcolo dell&apos;indicatore di salute quando l&apos;indicatore sanitario è  &apos;condizioni di salute generali&apos;.&apos;</rdfs:comment>
        <rdfs:comment xml:lang="en">The class of the indicator calculation related to the general health condition of the population. This class is equivalent to the &apos;health indicator calculation when the health indicator is &apos;general health conditions&apos;.&apos;</rdfs:comment>
        <rdfs:isDefinedBy rdf:resource="https://w3id.org/whow/onto/health-monitoring"/>
        <rdfs:label xml:lang="it">Calcolo dell&apos;Indicatore Condizioni di Salute Generali</rdfs:label>
        <rdfs:label xml:lang="en">Health Condition Indicator Calculation</rdfs:label>
        <owl:versionInfo xml:lang="it">provvisoria</owl:versionInfo>
        <owl:versionInfo xml:lang="en">unstable</owl:versionInfo>
    </owl:Class>



    <!-- https://w3id.org/whow/onto/health-monitoring/HealthOrganisation -->

    <owl:Class rdf:about="https://w3id.org/whow/onto/health-monitoring/HealthOrganisation">
        <rdfs:subClassOf rdf:resource="https://w3id.org/italia/env/onto/top/Organisation"/>
        <rdfs:comment xml:lang="en">A generic organisation operating in the healthcare context. This class includes organisations such as ASLs or in-patient facilities.</rdfs:comment>
        <rdfs:comment xml:lang="it">Una generica organizzazione che opera nel contesto sanitario. Questa classe include organizzazioni tipo le ASL o le strutture di ricovero.</rdfs:comment>
        <rdfs:isDefinedBy rdf:resource="https://w3id.org/whow/onto/health-monitoring"/>
        <rdfs:label xml:lang="en">Health Organisation</rdfs:label>
        <rdfs:label xml:lang="en">Organizzazione Sanitaria</rdfs:label>
        <owl:versionInfo xml:lang="it">stabile</owl:versionInfo>
        <owl:versionInfo xml:lang="en">stable</owl:versionInfo>
    </owl:Class>



    <!-- https://w3id.org/whow/onto/health-monitoring/HealthcareAuthority -->

    <owl:Class rdf:about="https://w3id.org/whow/onto/health-monitoring/HealthcareAuthority">
        <rdfs:subClassOf rdf:resource="https://w3id.org/whow/onto/health-monitoring/HealthOrganisation"/>
        <rdfs:subClassOf>
            <owl:Restriction>
                <owl:onProperty rdf:resource="https://w3id.org/whow/onto/health-monitoring/isTerritoriallyCompetentFor"/>
                <owl:allValuesFrom rdf:resource="https://w3id.org/whow/onto/health-monitoring/InpatientFacility"/>
            </owl:Restriction>
        </rdfs:subClassOf>
        <owl:disjointWith rdf:resource="https://w3id.org/whow/onto/health-monitoring/InpatientFacility"/>
        <rdfs:comment xml:lang="it">La classe delle organizzazioni specifiche che di solito in ambito territoriale si occupano di assistenza sanitaria (nel caso di Regione Lombardia sono le ATS, in altre regioni si chiamano ASL o AUSL). Queste hanno tipicamente le seguenti funzioni:
1) negoziazione e acquisto delle prestazioni sanitarie e sociosanitarie dalle strutture accreditate;
2) governo del percorso di presa in carico della persona in tutta la rete dei servizi sanitari, sociosanitari e sociali;
3) governo dell’assistenza primaria e del convenzionamento delle cure primarie;
4) governo e promozione dei programmi di educazione alla salute, prevenzione, assistenza, cura e riabilitazione;
5) promozione della sicurezza alimentare medica e medica veterinaria;
6) prevenzione e controllo della salute negli ambienti di vita e di lavoro, compreso il controllo periodico impiantistico e tecnologico;
7) sanità pubblica veterinaria;
8) attuazione degli indirizzi regionali e monitoraggio della spesa in materia di farmaceutica, dietetica e protesica;
9) vigilanza e controllo sulle strutture e sulle unità d’offerta sanitarie, sociosanitarie e sociali.</rdfs:comment>
        <rdfs:comment xml:lang="en">The class of specific organisations that usually deal with health care in a territorial context (in the case of the Lombardy Region they are named ATS, in other regions they are called ASL or AUSL). These typically have the following functions
1) negotiation and purchase of health and socio-health services from accredited facilities;
2) governance of the person&apos;s care pathway throughout the network of health, social and health services
3) governance of primary and contracted primary care;
4) governance and promotion of health education, prevention, care, treatment and rehabilitation programmes;
5) promotion of medical and veterinary food safety;
6) prevention and control of health in living and working environments, including periodic plant and technological control;
7) veterinary public health
8) implementation of regional guidelines and monitoring of expenditure on pharmaceuticals, dietetics and prosthetics;
9) supervision and control of healthcare, social and health facilities and units.</rdfs:comment>
        <rdfs:isDefinedBy rdf:resource="https://w3id.org/whow/onto/health-monitoring"/>
        <rdfs:label xml:lang="it">Agenzia/Azienda Sanitaria</rdfs:label>
        <rdfs:label xml:lang="en">Healthcare Authority</rdfs:label>
        <owl:versionInfo xml:lang="it">stabile</owl:versionInfo>
        <owl:versionInfo xml:lang="en">stable</owl:versionInfo>
    </owl:Class>



    <!-- https://w3id.org/whow/onto/health-monitoring/HealthcareIndicator -->

    <owl:Class rdf:about="https://w3id.org/whow/onto/health-monitoring/HealthcareIndicator">
        <rdfs:subClassOf rdf:resource="https://w3id.org/italia/env/onto/top/Entity"/>
        <rdfs:subClassOf>
            <owl:Restriction>
                <owl:onProperty rdf:resource="https://w3id.org/italia/env/onto/top/isClassifiedBy"/>
                <owl:allValuesFrom rdf:resource="https://w3id.org/whow/onto/health-monitoring/IndicatorType"/>
            </owl:Restriction>
        </rdfs:subClassOf>
        <rdfs:comment xml:lang="it">La classe degli indicatori di salute. Utilizzata per poter creare un vocabolario controllato di indicatori in questo settore applicativo.</rdfs:comment>
        <rdfs:comment xml:lang="en">The class of the health care indicator. It is used to create a controlled list of possible indicators to be used in the health sector.</rdfs:comment>
        <rdfs:isDefinedBy rdf:resource="https://w3id.org/whow/onto/health-monitoring"/>
        <rdfs:label xml:lang="en">Health Care Indicator</rdfs:label>
        <rdfs:label xml:lang="it">Indicatore di Salute</rdfs:label>
        <owl:versionInfo xml:lang="it">stabile</owl:versionInfo>
        <owl:versionInfo xml:lang="en">stable</owl:versionInfo>
    </owl:Class>



    <!-- https://w3id.org/whow/onto/health-monitoring/HealthcareIndicatorCalculation -->

    <owl:Class rdf:about="https://w3id.org/whow/onto/health-monitoring/HealthcareIndicatorCalculation">
        <rdfs:subClassOf rdf:resource="https://w3id.org/italia/env/onto/inspire-mf/Indicator"/>
        <rdfs:subClassOf rdf:resource="https://w3id.org/italia/env/onto/top/Eventuality"/>
        <rdfs:subClassOf>
            <owl:Restriction>
                <owl:onProperty rdf:resource="https://w3id.org/italia/env/onto/top/atTime"/>
                <owl:someValuesFrom rdf:resource="https://w3id.org/italia/env/onto/top/TemporalEntity"/>
            </owl:Restriction>
        </rdfs:subClassOf>
        <rdfs:subClassOf>
            <owl:Restriction>
                <owl:onProperty rdf:resource="https://w3id.org/whow/onto/health-monitoring/hasHealthcareIndicatorValue"/>
                <owl:someValuesFrom rdf:resource="https://w3id.org/italia/env/onto/top/Value"/>
            </owl:Restriction>
        </rdfs:subClassOf>
        <rdfs:subClassOf>
            <owl:Restriction>
                <owl:onProperty rdf:resource="https://w3id.org/italia/env/onto/inspire-mf/isIndicatorOf"/>
                <owl:allValuesFrom rdf:resource="https://w3id.org/whow/onto/health-monitoring/HealthOrganisation"/>
            </owl:Restriction>
        </rdfs:subClassOf>
        <rdfs:subClassOf>
            <owl:Restriction>
                <owl:onProperty rdf:resource="https://w3id.org/whow/onto/health-monitoring/ofClinicalCohort"/>
                <owl:allValuesFrom rdf:resource="https://w3id.org/whow/onto/health-monitoring/ClinicalCohort"/>
            </owl:Restriction>
        </rdfs:subClassOf>
        <rdfs:subClassOf>
            <owl:Restriction>
                <owl:onProperty rdf:resource="https://w3id.org/whow/onto/health-monitoring/subIndicator"/>
                <owl:allValuesFrom rdf:resource="https://w3id.org/whow/onto/health-monitoring/HealthcareIndicatorCalculation"/>
            </owl:Restriction>
        </rdfs:subClassOf>
        <rdfs:comment xml:lang="it">La classe che rappresenta il calcolo dell&apos;indicatore di salute e che quindi mette insieme l&apos;indicatore che viene calcolato, il valore risultante dal calcolo, la coorte clinica utilizzata in base a determinati criteri di suddivisione della popolazione e l&apos;area territoriale di pertinenza.</rdfs:comment>
        <rdfs:comment xml:lang="en">The class that represents the calculation of the health care indicator and thus brings together the indicator being calculated, the value resulting from the calculation, the clinical cohort used according to certain population breakdown criteria and the relevant territorial area.</rdfs:comment>
        <rdfs:isDefinedBy rdf:resource="https://w3id.org/whow/onto/health-monitoring"/>
        <rdfs:label xml:lang="it">Calcolo dell&apos;Indicatore di Salute</rdfs:label>
        <rdfs:label xml:lang="en">Healthcare Indicator Calculation</rdfs:label>
        <owl:versionInfo xml:lang="it">stabile</owl:versionInfo>
        <owl:versionInfo xml:lang="en">stable</owl:versionInfo>
    </owl:Class>



    <!-- https://w3id.org/whow/onto/health-monitoring/HospitalCareIndicatorCalculation -->

    <owl:Class rdf:about="https://w3id.org/whow/onto/health-monitoring/HospitalCareIndicatorCalculation">
        <rdfs:subClassOf rdf:resource="https://w3id.org/whow/onto/health-monitoring/HealthcareIndicatorCalculation"/>
        <rdfs:comment xml:lang="it">La classe del calcolo dell&apos;indicatore relativo all&apos;assistenza ospedaliera. Questa classe è equivalente al &apos;calcolo dell&apos;indicatore di salute quando l&apos;indicatore sanitario è  &apos;assistenza ospedaliera&apos;.&apos;</rdfs:comment>
        <rdfs:comment xml:lang="en">The class of the hospital care indicator calculation. This class is equivalent to the &apos;health indicator calculation when the health indicator is &apos;hospital care&apos;.&apos;</rdfs:comment>
        <rdfs:isDefinedBy rdf:resource="https://w3id.org/whow/onto/health-monitoring"/>
        <rdfs:label xml:lang="it">Calcolo Indicatore Assistenza Ospedaliera</rdfs:label>
        <rdfs:label xml:lang="en">Hospital Care Indicator Calculation</rdfs:label>
        <owl:versionInfo xml:lang="it">provvisoria</owl:versionInfo>
        <owl:versionInfo xml:lang="en">unstable</owl:versionInfo>
    </owl:Class>



    <!-- https://w3id.org/whow/onto/health-monitoring/IndicatorType -->

    <owl:Class rdf:about="https://w3id.org/whow/onto/health-monitoring/IndicatorType">
        <rdfs:subClassOf rdf:resource="https://w3id.org/italia/env/onto/top/Characteristic"/>
        <rdfs:subClassOf rdf:resource="https://w3id.org/italia/env/onto/top/Concept"/>
        <rdfs:comment xml:lang="it">La classe dei diversi tipi di indicatori. Tipicamente nel settore sanitario, i tipi di indicatori sono: indicatore di processo, indicatore di risultato, indicatore di struttura.</rdfs:comment>
        <rdfs:comment xml:lang="en">The class of the different types of indicators. Typically in the health care sector, types of indicators are: process indicator, outcome indicator, structure indicator.</rdfs:comment>
        <rdfs:isDefinedBy rdf:resource="https://w3id.org/whow/onto/health-monitoring"/>
        <rdfs:label xml:lang="en">Indicator Type</rdfs:label>
        <rdfs:label xml:lang="it">Tipo di Indicatore</rdfs:label>
        <owl:versionInfo xml:lang="it">stabile</owl:versionInfo>
        <owl:versionInfo xml:lang="en">stable</owl:versionInfo>
    </owl:Class>



    <!-- https://w3id.org/whow/onto/health-monitoring/InfectiousDiseaseIndicatorCalculation -->

    <owl:Class rdf:about="https://w3id.org/whow/onto/health-monitoring/InfectiousDiseaseIndicatorCalculation">
        <rdfs:subClassOf rdf:resource="https://w3id.org/whow/onto/health-monitoring/HealthcareIndicatorCalculation"/>
        <rdfs:comment xml:lang="en">La classe del calcolo dell&apos;indicatore relativo alla distribuzione delle malattie infettive. Questa classe è equivalente al &apos;calcolo dell&apos;indicatore di salute quando l&apos;indicatore sanitario è  &apos;diffusione delle malattie infettive&apos;.&apos;</rdfs:comment>
        <rdfs:comment xml:lang="en">The class of the specific calculation related to infectious diseases distribution. This class is equivalent to the Healthcare Indicator Calculation when the Healthcare Indicator is diffusion of infectious diseases.</rdfs:comment>
        <rdfs:isDefinedBy rdf:resource="https://w3id.org/whow/onto/health-monitoring"/>
        <rdfs:label xml:lang="it">Calcolo dell&apos;Indicatore Malattie Infettive</rdfs:label>
        <rdfs:label xml:lang="en">Infectious Disease Indicator Calculation</rdfs:label>
        <owl:versionInfo xml:lang="it">provvisoria</owl:versionInfo>
        <owl:versionInfo xml:lang="en">unstable</owl:versionInfo>
    </owl:Class>



    <!-- https://w3id.org/whow/onto/health-monitoring/InpatientFacility -->

    <owl:Class rdf:about="https://w3id.org/whow/onto/health-monitoring/InpatientFacility">
        <rdfs:subClassOf rdf:resource="https://w3id.org/whow/onto/health-monitoring/HealthOrganisation"/>
        <rdfs:comment xml:lang="en">Hospital care guarantees admission to accredited public and private hospitals for the diagnosis and treatment of acute or long-term illnesses that cannot be dealt with on an outpatient or home basis. The Ministry of Health, as part of the Health Information System
Health Information System collects information on public and private hospitalisation facilities and their activities (provenance: Italian Ministry of Health)</rdfs:comment>
        <rdfs:comment xml:lang="it">L’assistenza ospedaliera garantisce il ricovero presso gli ospedali pubblici e privati accreditati per la diagnosi e la cura delle malattie acute o di lunga durata che non possono essere affrontate ambulatorialmente o a domicilio. Il Ministero della Salute, nell’ambito del Sistema Informativo
Sanitario raccoglie informazioni sulla struttura di ricovero pubblica e privata e relative attività della struttura (fonte Ministero della salute)</rdfs:comment>
        <rdfs:isDefinedBy rdf:resource="https://w3id.org/whow/onto/health-monitoring"/>
        <rdfs:label xml:lang="en">Inpatient Facility</rdfs:label>
        <rdfs:label xml:lang="it">Struttura di Ricovero e Cura</rdfs:label>
        <owl:versionInfo xml:lang="it">stabile</owl:versionInfo>
        <owl:versionInfo xml:lang="en">stable</owl:versionInfo>
    </owl:Class>



    <!-- https://w3id.org/whow/onto/health-monitoring/Population -->

    <owl:Class rdf:about="https://w3id.org/whow/onto/health-monitoring/Population">
        <rdfs:subClassOf rdf:resource="https://w3id.org/italia/env/onto/top/Entity"/>
        <rdfs:subClassOf>
            <owl:Restriction>
                <owl:onProperty rdf:resource="https://w3id.org/whow/onto/health-monitoring/totalValue"/>
                <owl:maxQualifiedCardinality rdf:datatype="http://www.w3.org/2001/XMLSchema#nonNegativeInteger">1</owl:maxQualifiedCardinality>
                <owl:onDataRange rdf:resource="http://www.w3.org/2001/XMLSchema#float"/>
            </owl:Restriction>
        </rdfs:subClassOf>
        <rdfs:comment xml:lang="it">La classe che rappresenta la popolazione (di una regione in questa ontologia) totale, utilizzata nel calcolo degli indicatori di salute.</rdfs:comment>
        <rdfs:comment xml:lang="en">The class of the entire popolation considered when computing specific healthcare indicator calculation operations</rdfs:comment>
        <rdfs:isDefinedBy rdf:resource="https://w3id.org/whow/onto/health-monitoring"/>
        <rdfs:label xml:lang="it">Popolazione</rdfs:label>
        <rdfs:label xml:lang="en">Population</rdfs:label>
        <owl:versionInfo xml:lang="it">stabile</owl:versionInfo>
        <owl:versionInfo xml:lang="en">stable</owl:versionInfo>
    </owl:Class>
</rdf:RDF>



<!-- Generated by the OWL API (version 4.5.9.2019-02-01T07:24:44Z) https://github.com/owlcs/owlapi -->
